WIP: first case

dataplane/Examples/Batch_op_Correctness.thy
@@ -22,91 +22,6 @@ abbreviation "t_1_0 \<equiv> MyPair (Suc 0) (0 :: nat)"
 abbreviation "t_0_1 \<equiv> MyPair (0 :: nat) (Suc 0)"
 abbreviation "t_1_1 \<equiv> MyPair (Suc 0) (Suc 0)"
 
-abbreviation "list_inps_test \<equiv> 
- [Mint t_1_0, Mint t_0_1, Mint t_1_1, Drop t0, Data t_1_1 10, Drop t_1_1, Data t_0_1 7, Data t_1_0 (3 :: nat), Drop t_1_0, Drop t_0_1]"
-abbreviation "inps_test \<equiv> llist_of list_inps_test"
-
-abbreviation init_input_state where
-  "init_input_state su inps \<equiv> \<lparr> 
-   summar = su,
-   consu = [],
-   inter = [],
-   produ = [],
-   input = (\<lambda> _. []),
-   outpu = (\<lambda> _. []),
-   front = undefined,
-   ocaps = (\<lambda> _. [0]),
-   initia = False,
-   nfron = False,
-   en1 = Inl,
-   de1 = projl,
-   es = inps
-   \<rparr>"
-abbreviation init_operator_state_ty2 where
-  "init_operator_state_ty2 su \<equiv> \<lparr> 
-   summar = su,
-   consu = [],
-   inter = [],
-   produ = [],
-   input = (\<lambda> _. []),
-   outpu = (\<lambda> _. []),
-   front = undefined,
-   ocaps = (\<lambda> _. []),
-   initia = False,
-   nfron = False,
-   en1 = Inl,
-   de1 = projl,
-   en2 = Inr,
-   de2 = projr
-   \<rparr>"
-
-abbreviation "l1 ip_state \<equiv> ((Logic (ooo_input_op {|1 :: 1|} ip_state) default_internal_summary) :: ('a, _, (_, 't) shared_state + (1 \<Rightarrow> 't antichain), 'c \<times> 't, 't :: {ccompare,canonically_ordered_monoid_add,ordered_ab_semigroup_monoid_add_imp_le,bot}) dataflow_tree)"
-abbreviation "l2 os2 f \<equiv> Logic (batch_op os2 f) default_internal_summary"
-abbreviation "G f ip_state os2 \<equiv> Comp [(0 :: 2, 1) \<mapsto> (0, 1)] (l1 (ip_state :: (1, 'd1 + 'd2, 'd1, _) input_state)) (l2 (os2 :: (1, 'd1 + 'd2, 'd1, 'd2, _) operator_state_ty2) f)"
-
-abbreviation "test_op \<equiv> compile_dataflow (\<lambda> _. []) (G (\<lambda> b. if b = [] then trace (STR ''Empty batch! ! !'') [] else [Max (set b)]) (init_input_state default_internal_summary (\<lambda> _. inps_test)) (init_operator_state_ty2 default_internal_summary) )"
-
-value [GHC] "lmap (\<lambda> io. case io of VOut p (x, t) \<Rightarrow> (projr x, t)) (trace_exec test_op)"
-value [GHC] "check_prefix 100 [((1, 1), (Inr 10, MyPair 1 1)), ((1, 1), (Inr 7, MyPair 0 1)),((1, 1), (Inr 3, MyPair 1 0))] test_op"
-value [GHC] "check_prefix 100 [((1, 1), (Inr 7, MyPair 0 1)), ((1, 1), (Inr 10, MyPair 1 1)), ((1, 1), (Inr 3, MyPair 1 0))] test_op"
-value [GHC] "check_prefix 100 [((1, 1), (Inr 3, MyPair 1 0)), ((1, 1), (Inr 10, MyPair 1 1)), ((1, 1), (Inr 7, MyPair 0 1))] test_op"
-
-section \<open>Generalized Correctness\<close>
-
-abbreviation "coll inps t \<equiv> list_of (lmap (\<lambda> e. case e of Data t d \<Rightarrow> d) (lfilter (\<lambda> e. case e of Data t' d \<Rightarrow> t = t' | _ \<Rightarrow> False) inps))"
-
-abbreviation "ts inps \<equiv> cimage (\<lambda> e. case e of Data t d \<Rightarrow> t) (cfilter is_Data (cset_of_llist inps))"
-
-abbreviation "inp_op os \<equiv> map_op (case_option (Inl (0 :: 2)) (\<lambda> p. Inr (0, p))) (case_option (Inl (0 :: 2)) (\<lambda> p. Inr (0, p))) (ooo_input_op {|1|} os)"
-abbreviation "tt_op os f \<equiv> map_op (case_option (Inl (1 :: 2)) (\<lambda> p. Inr (1, p))) (case_option (Inl (1 :: 2)) (\<lambda> p. Inr (1, p))) (batch_op os f)"
-
-abbreviation "G_op f ip_state os2 chns \<equiv>
-   dataflow_tree_to_operator chns (G f (ip_state :: (1, 'd1 + 'd2, 'd1, _) input_state) (os2 :: (1, 'd1 + 'd2, 'd1, 'd2, _) operator_state_ty2))"
-
-definition "c_pts_inv c caps = (\<forall> l. c_pts c l = caps l)"
-definition "Src_caps_inv caps oss = (\<forall> nid p. caps (Loc nid (Src p)) = zmset_of (mset (ocaps (oss nid) p)))"
-definition "Trg_caps_inv caps bufs = (\<forall> nid p. caps (Loc nid (Trg p)) = zmset_of (mset (map snd (bufs nid p))))"
-definition "extract_prog eds oss = concat (map (\<lambda> nid. extract_progress nid eds (snd (obtain_progress (oss nid)))) Enum.enum)"
-definition "front_inv oss c = (\<forall> nid p. front (oss nid) p \<le> frontier (c_imp c (Loc nid (Trg p))))"
-definition "imp_front_inv su c = (\<forall> l. frontier (c_imp c l) \<le> ifrontier su (+) c l)"
-definition "chnls_imp_front_inv su c chns = (\<forall> nid p. \<forall> t \<in> snd ` set (chns (nid, p)). frontier_less_equal (ifrontier su (+) c (Loc nid (Trg p))) t)"
-
-definition "propagation_inv su c = 
-  (dataflow_topology.inv_imps_work_sum su (-+-) c \<and>
-   dataflow_topology.inv_implications_nonneg c \<and>
-   dataflow_topology.inv_imp_plus_work_nonneg c)"
-
-definition "changes_non_zero_inv cgs = (\<forall>d\<in>snd ` snd ` set cgs. d \<noteq> 0)"
-definition "changes_above_impl_inv su c cgs = 
-  ((\<forall>(l, t, d)\<in>set cgs. frontier_less_equal (ifrontier su (+) c l) t) \<and>
-   (\<forall> l' \<in> fst ` set cgs. let (cgs_l, cgs') = partition (\<lambda> (l, t, d). l' = l) cgs in
-                         (\<forall> (l, t, d) \<in> set cgs'. frontier_less_equal (ifrontier su (+) (change_multiplicities su cgs_l c) l) t)))"
-
-abbreviation "su_test a b \<equiv> dataflow_tree_to_graph (
-    Comp [(0, 0) \<mapsto> (1, 1), (1, 0) \<mapsto> (0, 0)] 
-    (Comp [(0, 0) \<mapsto> (0, 0)] (Logic (\<oslash> :: (_, _, unit + unit) op) (\<lambda> _ _. [0 :: nat])) (Logic \<oslash> (\<lambda> _ _. [0 :: nat])))
-    (Comp [(0 :: 4, 0 :: 2) \<mapsto> (0, 0)] (Logic \<oslash> (\<lambda> _ _. [0 :: nat])) (Logic \<oslash> (\<lambda> _ _. [0 :: nat])))
-    ) a b"
 
 definition "my_summ = (\<lambda> l1 l2.
    if l1 = Loc (0 :: 2) (Src (0 :: 1)) \<and> l2 = Loc (1 :: 2)  (Trg (0 :: 1)) 
@@ -116,8 +31,6 @@ definition "my_summ = (\<lambda> l1 l2.
    else if l1 = Loc 1 (Trg 0) \<and> l2 = Loc 1 (Src 0)
    then antichain_from_list [0]
    else {}\<^sub>A)"
-
-term remove_non_zero_weights
 
 lemma weights_to_graph_fun_to_next[simp]:
   "weights_to_graph_fun
@@ -137,12 +50,13 @@ lemma weights_to_graph_fun_to_next[simp]:
   subgoal for l
     using loc_2_1_cases[where l=l] apply -
     apply (elim disjE; hypsubst_thin)
-      apply (auto 0 0 simp add: antichain_empty set_antichain1 antichain_from_list_empty enum_location_def enum_port_def Numeral_Type.enum_num1_def comp_def Enum.enum_prod_def split: sum.splits option.splits sum.splits)
+       apply (auto 0 0 simp add: antichain_empty set_antichain1 antichain_from_list_empty enum_location_def enum_port_def Numeral_Type.enum_num1_def comp_def Enum.enum_prod_def split: sum.splits option.splits sum.splits)
     using not_in_empty apply blast+
-       apply code_simp
+      apply code_simp
     using not_in_empty apply blast+
     done
   done
+
 
 lemma dataflow_tree_to_graph_to_my_summ[simp]:
   "dataflow_tree_to_graph (Comp [(0, 1) \<mapsto> (0, 1)] (Logic op1 default_internal_summary) (Logic op2 default_internal_summary)) = (my_summ :: (2, 1) location \<Rightarrow> (2, 1) location \<Rightarrow> _ antichain)"
@@ -184,261 +98,452 @@ lemma dataflow_tree_to_graph_to_my_summ[simp]:
     done
   done
 
+abbreviation "list_inps_test \<equiv> 
+ [Mint t_1_0, Mint t_0_1, Mint t_1_1, Drop t0, Data t_1_1 10, Drop t_1_1, Data t_0_1 7, Data t_1_0 (3 :: nat), Drop t_1_0, Drop t_0_1]"
+abbreviation "inps_test \<equiv> llist_of list_inps_test"
+
+abbreviation init_input_state where
+  "init_input_state su inps \<equiv> \<lparr> 
+   summar = su,
+   consu = [],
+   inter = [],
+   produ = [],
+   input = (\<lambda> _. []),
+   outpu = (\<lambda> _. []),
+   front = undefined,
+   ocaps = (\<lambda> _. [0]),
+   initia = False,
+   nfron = False,
+   en1 = Inl,
+   de1 = projl,
+   es = inps
+   \<rparr>"
+abbreviation init_operator_state_ty2 where
+  "init_operator_state_ty2 su \<equiv> \<lparr> 
+   summar = su,
+   consu = [],
+   inter = [],
+   produ = [],
+   input = (\<lambda> _. []),
+   outpu = (\<lambda> _. []),
+   front = undefined,
+   ocaps = (\<lambda> _. []),
+   initia = False,
+   nfron = False,
+   en1 = Inl,
+   de1 = projl,
+   en2 = Inr,
+   de2 = projr
+   \<rparr>"
+
+
+
+abbreviation "l1 ip_state \<equiv> ((Logic (ooo_input_op {|1 :: 1|} ip_state) default_internal_summary) :: ('a, _, (_, 't) shared_state + (1 \<Rightarrow> 't antichain), 'c \<times> 't, 't :: {ccompare,canonically_ordered_monoid_add,ordered_ab_semigroup_monoid_add_imp_le,bot}) dataflow_tree)"
+abbreviation "l2 os2 f \<equiv> Logic (batch_op os2 f) default_internal_summary"
+abbreviation "G f ip_state os2 \<equiv> Comp [(0 :: 2, 1) \<mapsto> (0, 1)] (l1 (ip_state :: (1, 'd1 + 'd2, 'd1, _) input_state)) (l2 (os2 :: (1, 'd1 + 'd2, 'd1, 'd2, _) operator_state_ty2) f)"
+
+abbreviation "test_op \<equiv> compile_dataflow (\<lambda> _. []) (G (\<lambda> b. if b = [] then trace (STR ''Empty batch! ! !'') [] else [Max (set b)]) (init_input_state default_internal_summary (\<lambda> _. inps_test)) (init_operator_state_ty2 default_internal_summary) )"
+
+value [GHC] "lmap (\<lambda> io. case io of VOut p (x, t) \<Rightarrow> (projr x, t)) (trace_exec test_op)"
+value [GHC] "check_prefix 100 [((1, 1), (Inr 10, MyPair 1 1)), ((1, 1), (Inr 7, MyPair 0 1)),((1, 1), (Inr 3, MyPair 1 0))] test_op"
+value [GHC] "check_prefix 100 [((1, 1), (Inr 7, MyPair 0 1)), ((1, 1), (Inr 10, MyPair 1 1)), ((1, 1), (Inr 3, MyPair 1 0))] test_op"
+value [GHC] "check_prefix 100 [((1, 1), (Inr 3, MyPair 1 0)), ((1, 1), (Inr 10, MyPair 1 1)), ((1, 1), (Inr 7, MyPair 0 1))] test_op"
+
+section \<open>Generalized Correctness\<close>
+
+abbreviation "coll inps t \<equiv> list_of (lmap (\<lambda> e. case e of Data t d \<Rightarrow> d) (lfilter (\<lambda> e. case e of Data t' d \<Rightarrow> t = t' | _ \<Rightarrow> False) inps))"
+
+abbreviation "ts inps \<equiv> cimage (\<lambda> e. case e of Data t d \<Rightarrow> t) (cfilter is_Data (cset_of_llist inps))"
+
+abbreviation "inp_op os \<equiv> map_op (case_option (Inl (0 :: 2)) (\<lambda> p. Inr (0, p))) (case_option (Inl (0 :: 2)) (\<lambda> p. Inr (0, p))) (ooo_input_op {|1|} os)"
+abbreviation "tt_op os f \<equiv> map_op (case_option (Inl (1 :: 2)) (\<lambda> p. Inr (1, p))) (case_option (Inl (1 :: 2)) (\<lambda> p. Inr (1, p))) (batch_op os f)"
+
+abbreviation "G_op f ip_state os2 chns \<equiv>
+   dataflow_tree_to_operator chns (G f (ip_state :: (1, 'd1 + 'd2, 'd1, _) input_state) (os2 :: (1, 'd1 + 'd2, 'd1, 'd2, _) operator_state_ty2))"
+
+definition "c_pts_inv c caps = (\<forall> l. c_pts c l = caps l)"
+definition "Src_caps_inv caps os = (\<forall> nid p. caps (Loc nid (Src p)) = zmset_of (mset (ocaps (os nid) p)))"
+definition "Trg_caps_inv caps bufs = (\<forall> nid p. caps (Loc nid (Trg p)) = zmset_of (mset (map snd (bufs (nid, p)))))"
+definition "extract_prog eds os = concat (map (\<lambda> nid. extract_progress nid eds (snd (obtain_progress (os nid)))) Enum.enum)"
+definition "front_inv os c = (\<forall> nid p. front (os nid) p \<le> frontier (c_imp c (Loc nid (Trg p))))"
+definition "imp_front_inv su c = (\<forall> l. frontier (c_imp c l) \<le> ifrontier su (+) c l)"
+definition "chnls_imp_front_inv su c chns = (\<forall> nid p. \<forall> t \<in> snd ` set (chns (nid, p)). frontier_less_equal (ifrontier su (+) c (Loc nid (Trg p))) t)"
+
+definition "propagation_inv su c = 
+  (dataflow_topology.inv_imps_work_sum su (-+-) c \<and>
+   dataflow_topology.inv_implications_nonneg c \<and>
+   dataflow_topology.inv_imp_plus_work_nonneg c)"
+
+definition "changes_non_zero_inv cgs = (\<forall>d\<in>snd ` snd ` set cgs. d \<noteq> 0)"
+definition "changes_above_impl_inv su c cgs = 
+  ((\<forall>(l, t, d)\<in>set cgs. frontier_less_equal (ifrontier su (+) c l) t) \<and>
+   (\<forall> l' \<in> fst ` set cgs. let (cgs_l, cgs') = partition (\<lambda> (l, t, d). l' = l) cgs in
+                         (\<forall> (l, t, d) \<in> set cgs'. frontier_less_equal (ifrontier su (+) (change_multiplicities su cgs_l c) l) t)))"
+
+abbreviation "su_test a b \<equiv> dataflow_tree_to_graph (
+    Comp [(0, 0) \<mapsto> (1, 1), (1, 0) \<mapsto> (0, 0)] 
+    (Comp [(0, 0) \<mapsto> (0, 0)] (Logic (\<oslash> :: (_, _, unit + unit) op) (\<lambda> _ _. [0 :: nat])) (Logic \<oslash> (\<lambda> _ _. [0 :: nat])))
+    (Comp [(0 :: 4, 0 :: 2) \<mapsto> (0, 0)] (Logic \<oslash> (\<lambda> _ _. [0 :: nat])) (Logic \<oslash> (\<lambda> _ _. [0 :: nat])))
+    ) a b"
+
+
 definition Src_from_Trg where
   "Src_from_Trg su nid p = {(nid', p'). su (Loc nid' (Src p')) (Loc nid (Trg p)) \<noteq> {}\<^sub>A}"
 
-definition "outputs_at_target su oss = (\<lambda> (nid, p). let S = Src_from_Trg su nid p in if S = {} then [] else let (nid', p') = Set.the_elem S in outpu (oss nid') p')"
+definition "outputs_at_target su os = (\<lambda> (nid, p). let S = Src_from_Trg su nid p in if S = {} then [] else let (nid', p') = Set.the_elem S in outpu (os nid') p')"
+definition "inputs_at_target os = (\<lambda> (nid, p). input (os nid) p)"
+
+lemma outputs_at_target_consumes[simp]:
+  "outputs_at_target su (os(nid := consumes (os nid) p' t d)) = outputs_at_target su os"
+  unfolding outputs_at_target_def consumes_def Src_from_Trg_def add_caps_def
+  apply (rule ext)+
+  apply (auto split: if_splits prod.splits)
+  done
+
 
 definition "all_isl l = (\<forall> x \<in> fst ` set l. isl x)"
 
-definition "INVAR plane_state tracker_state = 
-   (\<exists> oss :: 'nid \<Rightarrow> ('p, 'd, 't) operator_state.
-    True)"
+definition "dataplane_tracker_inv os cbufs sg Pcaps = 
+   (\<exists> c c' cgs chns caps.
+     c = pt_tr sg \<and>
+     cgs = extract_prog (edges sg) os \<and>
+     chns = outputs_at_target (summ sg) os >> cbufs >> inputs_at_target os \<and>
+     Src_caps_inv caps os \<and>
+     Trg_caps_inv caps cbufs \<and>
+     cgs = extract_prog (edges sg) os \<and>
+     c' = change_multiplicities (summ sg) cgs c \<and>
+     c_pts_inv c' caps \<and>
+     front_inv os c \<and>
+     imp_front_inv (summ sg) c \<and>
+     chnls_imp_front_inv (summ sg) c chns \<and>
+     changes_non_zero_inv cgs \<and>
+     propagation_inv (summ sg) c \<and>
+     Pcaps caps)"
 
 lemma correctness_gen:
   fixes inps :: \<open>1 \<Rightarrow> ('t :: {ccompare,canonically_ordered_monoid_add,ordered_ab_semigroup_monoid_add_imp_le,bot}, 'd1) event llist\<close>
     and f :: \<open>'d1 buf \<Rightarrow> 'd2 buf\<close>
     and ip_state :: \<open>(1, 'd1 + 'd2, 'd1, 't) input_state\<close>
     and bt_state :: \<open>(1, 'd1 + 'd2, 'd1, 'd2, 't) operator_state_ty2\<close>
-    and oss :: \<open>2 \<Rightarrow> (1, 'd1 + 'd2, 't) operator_state\<close>
+    and os :: \<open>2 \<Rightarrow> (1, 'd1 + 'd2, 't) operator_state\<close>
     and chns :: \<open>2 \<times> 1 \<Rightarrow> (('d1 + 'd2) \<times> 't) list\<close>
     and sg :: \<open>(2, 1, 't) subgraph\<close>
-    and caps :: \<open>(2, 1) location \<Rightarrow> 't zmultiset\<close>
   assumes
     SUBGRAPH_INV:
-    \<open>c = pt_tr sg\<close>
     \<open>summ sg = dataflow_tree_to_graph (G f ip_state bt_state)\<close>
     \<open>edges sg = graph_to_edges (summ sg)\<close>
     and
     OP_STATE_INV: 
-    \<open>ip_state = operator_state.extend (oss 0) \<lparr>en1 = Inl, de1 = projl, es = inps\<rparr>\<close>
-    \<open>bt_state = operator_state.extend (oss 1) \<lparr>en1 = Inl, de1 = projl, en2 = Inr, de2 = projr\<rparr>\<close>
-    and
-    BUFS_INV: 
-    \<open>outchns = outputs_at_target (summ sg) oss\<close>
-    \<open>inpchns = (\<lambda> (nid, p). input (oss nid) p)\<close>
-    \<open>chns = outchns >> cbufs >> inpchns\<close>
+    \<open>ip_state = operator_state.extend (os 0) \<lparr>en1 = Inl, de1 = projl, es = inps\<rparr>\<close>
+    \<open>bt_state = operator_state.extend (os 1) \<lparr>en1 = Inl, de1 = projl, en2 = Inr, de2 = projr\<rparr>\<close>
     \<open>all_isl (chns (0, 0))\<close>
     and
-    C_PTS_INV:
-    \<open>Src_caps_inv caps oss\<close>
-    \<open>Trg_caps_inv caps bufs\<close>
-    \<open>cgs = extract_prog (edges sg) oss\<close>
-    \<open>c' = change_multiplicities (summ sg) cgs c\<close>
-    \<open>c_pts_inv c' caps\<close>
+    BUFS_INV: 
+    \<open>chns = outputs_at_target (summ sg) os >> cbufs >> inputs_at_target os\<close>
     and
-    C_IMP_INV:
-    \<open>front_inv oss c\<close>
-    \<open>imp_front_inv (summ sg) c\<close>
-    \<open>chnls_imp_front_inv (summ sg) c chns\<close>
-    and
-    CGS_INV:
-    \<open>changes_above_impl_inv (summ sg) c cgs\<close>
-    \<open>changes_non_zero_inv cgs\<close>
-    and
-    PROP_INV:
-    \<open>propagation_inv (summ sg) c\<close>
-    and
-    INP_STREAM_INV:
-    \<open>timely_input_stream (inps 0) C\<close>
-    \<open>zmset_of C = caps (Loc 0 (Src 0))\<close>
+    DT_INV:
+    \<open>dataplane_tracker_inv os cbufs sg Pcaps\<close>
     and S_INV:
     \<open>SP = cUnion (cimage 
       (\<lambda> t. (cset_of_llist o llist_of) (map (\<lambda> x. ((2, 1), (Inr x, t))) (f (coll ((map (\<lambda> (x, t). Data t (projl x)) (chns (0, 0))) @@- (inps 1)) t))))
       (cUn (ts (inps 1)) (cset_of_llist (llist_of (map snd (chns (0, 0)))))))\<close>
-    \<open>SO = cset_of_llist (llist_of (outpu (os 1) 0))\<close>
+    \<open>SO = cset_of_llist (llist_of (map (\<lambda> x. ((2, 1), x)) (outpu (os 1) 0)))\<close>
+    and
+    INP_STREAM_INV:
+    \<open>Pcaps = (\<lambda> caps. timely_input_stream (inps 0) C \<and> zmset_of C = caps (Loc 0 (Src 0)))\<close>
   shows 
     \<open>set_op S D (dataflow_op sg (G_op f ip_state bt_state cbufs)) \<approx> set_spec_op (cUn (cUn S SO) SP) D\<close>
   using assms apply -
-proof (coinduction arbitrary: sg c c' cgs os ip_state bt_state oss chns cbufs bufs outchns inpchns caps C inps SP SO S D rule: weakBisimWeakUptoBisimCong)
+proof (coinduction arbitrary: os sg ip_state bt_state chns cbufs inps SP SO S D C Pcaps rule: weakBisimWeakUptoBisimCong)
   case SIM1
   show ?case (is "wsim ((~) OO \<U> ?R OO (\<approx>)) ?op1 ?op2")
   proof -
     define R where "R = ?R"
     show ?thesis 
-        apply -
-        unfolding R_def[symmetric]
-        subgoal premises prems2
-          unfolding wsim_def dataflow_tree_to_operator_def batch_op_def batch_op_logic_def ooo_input_op_def ooo_input_op_logic_def notifier_op_def
-          apply simp
-          apply (simp only: trace_simp)
-          apply (intro allI conjI impI)
-          apply (elim step_builder_op_elim step_set_op_elim step_map_op_elim step_comp_op_elim step_dataflow_op_elim conjE ; 
-              clarsimp simp only: IO.simps ; hypsubst_thin ? ; clarsimp simp flip: cin.rep_eq split: option.splits sum.splits prod.splits if_splits ; hypsubst_thin?)
-          subgoal 
-            apply -
-            apply (intro exI conjI relcomppI)
-               apply (rule step_set_spec_op_intro_Out)
-                  apply (rule refl)
-                 apply simp
-                apply simp
-               apply (rule refl)
-              apply (rule bisim_refl)
-             defer
-             apply (rule wbisim_refl)
-            apply (rule wb_upto_b_base)
-            unfolding R_def[simplified]
-            apply (intro exI conjI)
-            unfolding wsim_def dataflow_tree_to_operator_def batch_op_def batch_op_logic_def ooo_input_op_def ooo_input_op_logic_def notifier_op_def
-                                apply simp
-                                apply (simp only: trace_simp)
-                            apply (simp add: SIM1)
-                            apply (simp add: SIM1)
-                            apply (simp add: SIM1)
-                            apply (simp add: SIM1)
-        subgoal
-          using SIM1(7,8,9,2)
-          by (auto simp add: all_isl_def Src_from_Trg_def my_summ_def BULK_BENQ_def outputs_at_target_def split: prod.splits)
-        using SIM1(10) apply blast
-        using SIM1(11) apply blast
-        using SIM1 apply force+
-        done
-
-        find_theorems edges
-
-
-end
-        using SIM1(1,12,13,14) apply -
+      apply -
+      unfolding R_def[symmetric]
+      subgoal premises prems2
+        unfolding wsim_def dataflow_tree_to_operator_def batch_op_def batch_op_logic_def ooo_input_op_def ooo_input_op_logic_def notifier_op_def
         apply simp
-        apply hypsubst_thin
-
-
-        find_theorems c
-
-        defer
-                            defer
-                            defer
-                            defer
-                            defer
-        defer
-
-
-                         apply (simp_all only: SIM1 dataflow_tree_to_graph_to_my_summ)
-                        defer
-        using SIM1(21) apply simp
-        using SIM1(1,20) apply simp
-                      defer
-                      defer
-        defer
-        using SIM1(1,16) apply simp
-        using SIM1(1,15) apply simp
-        using SIM1(22) apply simp
-
-        find_theorems graph_to_edges
-
-end
-
-                        apply (rule arg_cong[where f="cUnion"])
-                        apply (rule arg_cong2[where f="cimage"])
-                         apply (rule ext)+
-        apply (simp split: prod.splits)
-         apply (rule refl)
-
-
-
-end
-      moreover have "\<exists>op2'. (step Tau)\<^sup>*\<^sup>* (set_spec_op (cUn (cUn S SO) SP) D) op2' \<and> ((~) OO \<U> R OO (\<approx>)) (set_op S D (dataflow_op sg (map_op (case_sum id id) (case_sum id id) (comp_op (case_sum (\<lambda>_. None) ((case_option None (Some \<circ> Inr) \<circ>\<circ> case_prod) (\<lambda>nid p. case if nid = 0 then Some (0, 1) else None of None \<Rightarrow> None | Some (offset, q) \<Rightarrow> Some (1 + offset, q)))) (case_sum (\<lambda>x. []) (BENQ (1, 1) (Inr (a, b)) (\<lambda>x. map Inr (cbufs x)))) (map_op (case_option (Inl 0) (\<lambda>p. Inr (0, 1))) (case_option (Inl 0) (\<lambda>p. Inr (0, 1))) (builder_op False {||} {|1|} (ip_state\<lparr>outpu := (outpu ip_state)(1 := xs)\<rparr>) (ooo_input_op_logic {|1|}))) (map_op (case_option (Inl 1) (\<lambda>p. Inr (1, 1))) (case_option (Inl 1) (\<lambda>p. Inr (1, 1))) (builder_op True {|1|} {|1|} (bt_state\<lparr>nfron := False\<rparr>) (\<lambda>os. if nfron os then if filter (\<lambda>t. \<not> frontier_less_equal (front os 1) t) (ocaps os 1) = [] then trace STR ''No capabilities'' {||} else let compl_batches = \<lambda>p t. map (de1 (os\<lparr>nfron := False\<rparr>) \<circ> fst) (filter (\<lambda>(d, t'). t' = t \<and> t \<in> set (filter (\<lambda>t. \<not> frontier_less_equal (front os p) t) (ocaps os p))) (input (os\<lparr>nfron := False\<rparr>) p)); ts = \<lambda>p. rmdups {} (map snd (filter (\<lambda>(d, t). t \<in> set (filter (\<lambda>t. \<not> frontier_less_equal (front os p) t) (ocaps os p))) (input (os\<lparr>nfron := False\<rparr>) p))); osa = os\<lparr>nfron := False, input := \<lambda>p. filter (\<lambda>(d, t). t \<notin> set (filter (\<lambda>t. \<not> frontier_less_equal (front os p) t) (ocaps os p))) (input (os\<lparr>nfron := False\<rparr>) p)\<rparr> in Let {|(concat (map (\<lambda>t. map (\<lambda>x. (x, Cap t 1)) (f (compl_batches 1 t))) (ts 1)), map (\<lambda>t. Cap t 1) (filter (\<lambda>t. \<not> frontier_less_equal (front os 1) t) (ocaps os 1)))|} ((|`|) (\<lambda>(outs, drops). trace (STR ''outs: '' + show_nat (length outs) + STR '' , drops: '' + show_nat (length drops)) (drop_caps (produces osa (map (\<lambda>(d, y). (en2 osa d, y)) outs)) drops))) else {||}))))))) op2'"
-        if "initia ip_state"
-          and "outpu ip_state 1 = (a, b) # xs"
-        for a :: "'d1 + 'd2"
-          and b :: 't
-          and xs :: "(('d1 + 'd2) \<times> 't) buf"
-        using that sorry
-      moreover have "\<exists>op2'. (step Tau)\<^sup>*\<^sup>* (set_spec_op (cUn (cUn S SO) SP) D) op2' \<and> ((~) OO \<U> R OO (\<approx>)) (set_op S D (dataflow_op sg (map_op (case_sum id id) (case_sum id id) (comp_op (case_sum (\<lambda>_. None) ((case_option None (Some \<circ> Inr) \<circ>\<circ> case_prod) (\<lambda>nid p. case if nid = 0 then Some (0, 1) else None of None \<Rightarrow> None | Some (offset, q) \<Rightarrow> Some (1 + offset, q)))) (case_sum (\<lambda>x. []) (BTL (1, 1) (\<lambda>x. map Inr (cbufs x)))) (map_op (case_option (Inl 0) (\<lambda>p. Inr (0, 1))) (case_option (Inl 0) (\<lambda>p. Inr (0, 1))) (builder_op False {||} {|1|} ip_state (ooo_input_op_logic {|1|}))) \<oslash>)))) op2'"
-        if "Inr (1, 1) \<in> ran (case_sum ((\<lambda>_. None)::2 \<Rightarrow> (2 + 2 \<times> 1) option) ((case_option None (Some \<circ> Inr) \<circ>\<circ> case_prod) (\<lambda>nid. (\<lambda>p. case if (nid::2) = 0 then Some (0, 1) else None of None \<Rightarrow> None | Some (offset, q) \<Rightarrow> Some (1 + offset, q))::1 \<Rightarrow> (_ \<times> _) option)))"
-          and "cbufs (1, 1) \<noteq> []"
-          and "initia bt_state"
-          and "is_Inl (BHD (1, 1) (\<lambda>x. map Inr (cbufs x))::((1, 't) shared_state + (1 \<Rightarrow> 't antichain)) + ('d1 + 'd2) \<times> 't)"
-        using that sorry
-      moreover have "\<exists>op2'. (step Tau)\<^sup>*\<^sup>* (set_spec_op (cUn (cUn S SO) SP) D) op2' \<and> ((~) OO \<U> R OO (\<approx>)) (set_op S D (dataflow_op sg (map_op (case_sum id id) (case_sum id id) (comp_op (case_sum (\<lambda>_. None) ((case_option None (Some \<circ> Inr) \<circ>\<circ> case_prod) (\<lambda>nid p. case if nid = 0 then Some (0, 1) else None of None \<Rightarrow> None | Some (offset, q) \<Rightarrow> Some (1 + offset, q)))) (case_sum (\<lambda>x. []) (BTL (1, 1) (\<lambda>x. map Inr (cbufs x)))) (map_op (case_option (Inl 0) (\<lambda>p. Inr (0, 1))) (case_option (Inl 0) (\<lambda>p. Inr (0, 1))) (builder_op False {||} {|1|} ip_state (ooo_input_op_logic {|1|}))) (map_op (case_option (Inl 1) (\<lambda>p. Inr (1, 1))) (case_option (Inl 1) (\<lambda>p. Inr (1, 1))) (builder_op True {|1|} {|1|} (consumes (bt_state\<lparr>nfron := False\<rparr>) 1 t d) (\<lambda>os. if nfron os then if filter (\<lambda>t. \<not> frontier_less_equal (front os 1) t) (ocaps os 1) = [] then trace STR ''No capabilities'' {||} else let compl_batches = \<lambda>p t. map (de1 (os\<lparr>nfron := False\<rparr>) \<circ> fst) (filter (\<lambda>(d, t'). t' = t \<and> t \<in> set (filter (\<lambda>t. \<not> frontier_less_equal (front os p) t) (ocaps os p))) (input (os\<lparr>nfron := False\<rparr>) p)); ts = \<lambda>p. rmdups {} (map snd (filter (\<lambda>(d, t). t \<in> set (filter (\<lambda>t. \<not> frontier_less_equal (front os p) t) (ocaps os p))) (input (os\<lparr>nfron := False\<rparr>) p))); osa = os\<lparr>nfron := False, input := \<lambda>p. filter (\<lambda>(d, t). t \<notin> set (filter (\<lambda>t. \<not> frontier_less_equal (front os p) t) (ocaps os p))) (input (os\<lparr>nfron := False\<rparr>) p)\<rparr> in Let {|(concat (map (\<lambda>t. map (\<lambda>x. (x, Cap t 1)) (f (compl_batches 1 t))) (ts 1)), map (\<lambda>t. Cap t 1) (filter (\<lambda>t. \<not> frontier_less_equal (front os 1) t) (ocaps os 1)))|} ((|`|) (\<lambda>(outs, drops). trace (STR ''outs: '' + show_nat (length outs) + STR '' , drops: '' + show_nat (length drops)) (drop_caps (produces osa (map (\<lambda>(d, y). (en2 osa d, y)) outs)) drops))) else {||}))))))) op2'"
-        if "Inr (1, 1) \<in> ran (case_sum ((\<lambda>_. None)::2 \<Rightarrow> (2 + 2 \<times> 1) option) ((case_option None (Some \<circ> Inr) \<circ>\<circ> case_prod) (\<lambda>nid. (\<lambda>p. case if (nid::2) = 0 then Some (0, 1) else None of None \<Rightarrow> None | Some (offset, q) \<Rightarrow> Some (1 + offset, q))::1 \<Rightarrow> (_ \<times> _) option)))"
-          and "cbufs (1, 1) \<noteq> []"
-          and "initia bt_state"
-          and "(Inr (d, t)::((1, 't) shared_state + (1 \<Rightarrow> 't antichain)) + ('d1 + 'd2) \<times> 't) = BHD (1, 1) (\<lambda>x. map Inr (cbufs x))"
-        for d :: "'d1 + 'd2"
-          and t :: 't
-        using that sorry
-      moreover have "\<exists>op2'. (step Tau)\<^sup>*\<^sup>* (set_spec_op (cUn (cUn S SO) SP) D) op2' \<and> ((~) OO \<U> R OO (\<approx>)) (set_op S D (dataflow_op sg (map_op (case_sum id id) (case_sum id id) (comp_op (case_sum (\<lambda>_. None) ((case_option None (Some \<circ> Inr) \<circ>\<circ> case_prod) (\<lambda>nid p. case if nid = 0 then Some (0, 1) else None of None \<Rightarrow> None | Some (offset, q) \<Rightarrow> Some (1 + offset, q)))) (case_sum (\<lambda>x. []) (\<lambda>x. map Inr (cbufs x))) (map_op (case_option (Inl 0) (\<lambda>p. Inr (0, 1))) (case_option (Inl 0) (\<lambda>p. Inr (0, 1))) (builder_op False {||} {|1|} os' (ooo_input_op_logic {|1|}))) (map_op (case_option (Inl 1) (\<lambda>p. Inr (1, 1))) (case_option (Inl 1) (\<lambda>p. Inr (1, 1))) (builder_op True {|1|} {|1|} (bt_state\<lparr>nfron := False\<rparr>) (\<lambda>os. if nfron os then if filter (\<lambda>t. \<not> frontier_less_equal (front os 1) t) (ocaps os 1) = [] then trace STR ''No capabilities'' {||} else let compl_batches = \<lambda>p t. map (de1 (os\<lparr>nfron := False\<rparr>) \<circ> fst) (filter (\<lambda>(d, t'). t' = t \<and> t \<in> set (filter (\<lambda>t. \<not> frontier_less_equal (front os p) t) (ocaps os p))) (input (os\<lparr>nfron := False\<rparr>) p)); ts = \<lambda>p. rmdups {} (map snd (filter (\<lambda>(d, t). t \<in> set (filter (\<lambda>t. \<not> frontier_less_equal (front os p) t) (ocaps os p))) (input (os\<lparr>nfron := False\<rparr>) p))); osa = os\<lparr>nfron := False, input := \<lambda>p. filter (\<lambda>(d, t). t \<notin> set (filter (\<lambda>t. \<not> frontier_less_equal (front os p) t) (ocaps os p))) (input (os\<lparr>nfron := False\<rparr>) p)\<rparr> in Let {|(concat (map (\<lambda>t. map (\<lambda>x. (x, Cap t 1)) (f (compl_batches 1 t))) (ts 1)), map (\<lambda>t. Cap t 1) (filter (\<lambda>t. \<not> frontier_less_equal (front os 1) t) (ocaps os 1)))|} ((|`|) (\<lambda>(outs, drops). trace (STR ''outs: '' + show_nat (length outs) + STR '' , drops: '' + show_nat (length drops)) (drop_caps (produces osa (map (\<lambda>(d, y). (en2 osa d, y)) outs)) drops))) else {||}))))))) op2'"
-        if "initia ip_state"
-          and "os' |\<in>| ooo_input_op_logic {|1|} ip_state"
-          and "ocaps ip_state 1 \<noteq> []"
-        for os' :: "(1, 'd1 + 'd2, 'd1, 't) input_state"
-        using that sorry
-      moreover have "\<exists>op2'. (step Tau)\<^sup>*\<^sup>* (set_spec_op (cUn (cUn S SO) SP) D) op2' \<and> ((~) OO \<U> R OO (\<approx>)) (set_op S D (dataflow_op (sg\<lparr>upfro := \<lambda>_. True, pt_tr := change_multiplicities (summ sg) (extract_progress 1 (edges sg) st) (pt_tr sg)\<rparr>) (map_op (case_sum id id) (case_sum id id) (comp_op (case_sum (\<lambda>_. None) ((case_option None (Some \<circ> Inr) \<circ>\<circ> case_prod) (\<lambda>nid p. case if nid = 0 then Some (0, 1) else None of None \<Rightarrow> None | Some (offset, q) \<Rightarrow> Some (1 + offset, q)))) (case_sum (\<lambda>x. []) (\<lambda>x. map Inr (cbufs x))) (map_op (case_option (Inl 0) (\<lambda>p. Inr (0, 1))) (case_option (Inl 0) (\<lambda>p. Inr (0, 1))) (builder_op False {||} {|1|} ip_state (ooo_input_op_logic {|1|}))) (map_op (case_option (Inl 1) (\<lambda>p. Inr (1, 1))) (case_option (Inl 1) (\<lambda>p. Inr (1, 1))) (builder_op True {|1|} {|1|} os' (\<lambda>os. if nfron os then if filter (\<lambda>t. \<not> frontier_less_equal (front os 1) t) (ocaps os 1) = [] then trace STR ''No capabilities'' {||} else let compl_batches = \<lambda>p t. map (de1 (os\<lparr>nfron := False\<rparr>) \<circ> fst) (filter (\<lambda>(d, t'). t' = t \<and> t \<in> set (filter (\<lambda>t. \<not> frontier_less_equal (front os p) t) (ocaps os p))) (input (os\<lparr>nfron := False\<rparr>) p)); ts = \<lambda>p. rmdups {} (map snd (filter (\<lambda>(d, t). t \<in> set (filter (\<lambda>t. \<not> frontier_less_equal (front os p) t) (ocaps os p))) (input (os\<lparr>nfron := False\<rparr>) p))); osa = os\<lparr>nfron := False, input := \<lambda>p. filter (\<lambda>(d, t). t \<notin> set (filter (\<lambda>t. \<not> frontier_less_equal (front os p) t) (ocaps os p))) (input (os\<lparr>nfron := False\<rparr>) p)\<rparr> in Let {|(concat (map (\<lambda>t. map (\<lambda>x. (x, Cap t 1)) (f (compl_batches 1 t))) (ts 1)), map (\<lambda>t. Cap t 1) (filter (\<lambda>t. \<not> frontier_less_equal (front os 1) t) (ocaps os 1)))|} ((|`|) (\<lambda>(outs, drops). trace (STR ''outs: '' + show_nat (length outs) + STR '' , drops: '' + show_nat (length drops)) (drop_caps (produces osa (map (\<lambda>(d, y). (en2 osa d, y)) outs)) drops))) else {||}))))))) op2'"
-        if "initia bt_state"
-          and "has_progress (bt_state\<lparr>nfron := False\<rparr>)"
-          and "(os', st) = obtain_progress (bt_state\<lparr>nfron := False\<rparr>)"
-        for st :: "(1, 't) shared_state"
-          and os' :: "(1, 'd1 + 'd2, 'd1, 'd2, 't) operator_state_ty2"
-        using that sorry
-      moreover have "\<exists>op2'. (step Tau)\<^sup>*\<^sup>* (set_spec_op (cUn (cUn S SO) SP) D) op2' \<and> ((~) OO \<U> R OO (\<approx>)) (set_op S D (dataflow_op (sg\<lparr>upfro := \<lambda>_. True, pt_tr := change_multiplicities (summ sg) (extract_progress 0 (edges sg) st) (pt_tr sg)\<rparr>) (map_op (case_sum id id) (case_sum id id) (comp_op (case_sum (\<lambda>_. None) ((case_option None (Some \<circ> Inr) \<circ>\<circ> case_prod) (\<lambda>nid p. case if nid = 0 then Some (0, 1) else None of None \<Rightarrow> None | Some (offset, q) \<Rightarrow> Some (1 + offset, q)))) (case_sum (\<lambda>x. []) (\<lambda>x. map Inr (cbufs x))) (map_op (case_option (Inl 0) (\<lambda>p. Inr (0, 1))) (case_option (Inl 0) (\<lambda>p. Inr (0, 1))) (builder_op False {||} {|1|} os' (ooo_input_op_logic {|1|}))) (map_op (case_option (Inl 1) (\<lambda>p. Inr (1, 1))) (case_option (Inl 1) (\<lambda>p. Inr (1, 1))) (builder_op True {|1|} {|1|} (bt_state\<lparr>nfron := False\<rparr>) (\<lambda>os. if nfron os then if filter (\<lambda>t. \<not> frontier_less_equal (front os 1) t) (ocaps os 1) = [] then trace STR ''No capabilities'' {||} else let compl_batches = \<lambda>p t. map (de1 (os\<lparr>nfron := False\<rparr>) \<circ> fst) (filter (\<lambda>(d, t'). t' = t \<and> t \<in> set (filter (\<lambda>t. \<not> frontier_less_equal (front os p) t) (ocaps os p))) (input (os\<lparr>nfron := False\<rparr>) p)); ts = \<lambda>p. rmdups {} (map snd (filter (\<lambda>(d, t). t \<in> set (filter (\<lambda>t. \<not> frontier_less_equal (front os p) t) (ocaps os p))) (input (os\<lparr>nfron := False\<rparr>) p))); osa = os\<lparr>nfron := False, input := \<lambda>p. filter (\<lambda>(d, t). t \<notin> set (filter (\<lambda>t. \<not> frontier_less_equal (front os p) t) (ocaps os p))) (input (os\<lparr>nfron := False\<rparr>) p)\<rparr> in Let {|(concat (map (\<lambda>t. map (\<lambda>x. (x, Cap t 1)) (f (compl_batches 1 t))) (ts 1)), map (\<lambda>t. Cap t 1) (filter (\<lambda>t. \<not> frontier_less_equal (front os 1) t) (ocaps os 1)))|} ((|`|) (\<lambda>(outs, drops). trace (STR ''outs: '' + show_nat (length outs) + STR '' , drops: '' + show_nat (length drops)) (drop_caps (produces osa (map (\<lambda>(d, y). (en2 osa d, y)) outs)) drops))) else {||}))))))) op2'"
-        if "initia ip_state"
-          and "has_progress ip_state"
-          and "(os', st) = obtain_progress ip_state"
-        for st :: "(1, 't) shared_state"
-          and os' :: "(1, 'd1 + 'd2, 'd1, 't) input_state"
-        using that sorry
-      moreover have "\<exists>op2'. (step Tau)\<^sup>*\<^sup>* (set_spec_op (cUn (cUn S SO) SP) D) op2' \<and> ((~) OO \<U> R OO (\<approx>)) (set_op S D (dataflow_op (sg\<lparr>pt_tr := x2, upfro := (upfro sg)(0 := False)\<rparr>) (map_op (case_sum id id) (case_sum id id) (comp_op (case_sum (\<lambda>_. None) ((case_option None (Some \<circ> Inr) \<circ>\<circ> case_prod) (\<lambda>nid p. case if nid = 0 then Some (0, 1) else None of None \<Rightarrow> None | Some (offset, q) \<Rightarrow> Some (1 + offset, q)))) (case_sum (\<lambda>x. []) (\<lambda>x. map Inr (cbufs x))) (map_op (case_option (Inl 0) (\<lambda>p. Inr (0, 1))) (case_option (Inl 0) (\<lambda>p. Inr (0, 1))) (builder_op False {||} {|1|} (ip_state \<lparr>front := frontier \<circ> (\<lambda>p. c_imp x2 (Loc 0 (Trg 1))), initia := True, nfron := True\<rparr>) (ooo_input_op_logic {|1|}))) (map_op (case_option (Inl 1) (\<lambda>p. Inr (1, 1))) (case_option (Inl 1) (\<lambda>p. Inr (1, 1))) (builder_op True {|1|} {|1|} (bt_state\<lparr>nfron := False\<rparr>) (\<lambda>os. if nfron os then if filter (\<lambda>t. \<not> frontier_less_equal (front os 1) t) (ocaps os 1) = [] then trace STR ''No capabilities'' {||} else let compl_batches = \<lambda>p t. map (de1 (os\<lparr>nfron := False\<rparr>) \<circ> fst) (filter (\<lambda>(d, t'). t' = t \<and> t \<in> set (filter (\<lambda>t. \<not> frontier_less_equal (front os p) t) (ocaps os p))) (input (os\<lparr>nfron := False\<rparr>) p)); ts = \<lambda>p. rmdups {} (map snd (filter (\<lambda>(d, t). t \<in> set (filter (\<lambda>t. \<not> frontier_less_equal (front os p) t) (ocaps os p))) (input (os\<lparr>nfron := False\<rparr>) p))); osa = os\<lparr>nfron := False, input := \<lambda>p. filter (\<lambda>(d, t). t \<notin> set (filter (\<lambda>t. \<not> frontier_less_equal (front os p) t) (ocaps os p))) (input (os\<lparr>nfron := False\<rparr>) p)\<rparr> in Let {|(concat (map (\<lambda>t. map (\<lambda>x. (x, Cap t 1)) (f (compl_batches 1 t))) (ts 1)), map (\<lambda>t. Cap t 1) (filter (\<lambda>t. \<not> frontier_less_equal (front os 1) t) (ocaps os 1)))|} ((|`|) (\<lambda>(outs, drops). trace (STR ''outs: '' + show_nat (length outs) + STR '' , drops: '' + show_nat (length drops)) (drop_caps (produces osa (map (\<lambda>(d, y). (en2 osa d, y)) outs)) drops))) else {||}))))))) op2'"
-        if "upfro sg 0"
-          and "\<not> initia ip_state"
-          and "propagate_all (summ sg) (pt_tr sg) = Some x2"
-        for x2 :: "((2, 1) location, 't) configuration"
-        using that sorry
-      moreover have "\<exists>op2'. (step Tau)\<^sup>*\<^sup>* (set_spec_op (cUn (cUn S SO) SP) D) op2' \<and> ((~) OO \<U> R OO (\<approx>)) (set_op S D (dataflow_op (sg\<lparr>pt_tr := x2, upfro := (upfro sg)(1 := False)\<rparr>) (map_op (case_sum id id) (case_sum id id) (comp_op (case_sum (\<lambda>_. None) ((case_option None (Some \<circ> Inr) \<circ>\<circ> case_prod) (\<lambda>nid p. case if nid = 0 then Some (0, 1) else None of None \<Rightarrow> None | Some (offset, q) \<Rightarrow> Some (1 + offset, q)))) (case_sum (\<lambda>x. []) (\<lambda>x. map Inr (cbufs x))) (map_op (case_option (Inl 0) (\<lambda>p. Inr (0, 1))) (case_option (Inl 0) (\<lambda>p. Inr (0, 1))) (builder_op False {||} {|1|} ip_state (ooo_input_op_logic {|1|}))) (map_op (case_option (Inl 1) (\<lambda>p. Inr (1, 1))) (case_option (Inl 1) (\<lambda>p. Inr (1, 1))) (builder_op True {|1|} {|1|} (bt_state \<lparr>front := frontier \<circ> (\<lambda>p. c_imp x2 (Loc 1 (Trg 1))), initia := True, nfron := True\<rparr>) (\<lambda>os. if nfron os then if filter (\<lambda>t. \<not> frontier_less_equal (front os 1) t) (ocaps os 1) = [] then trace STR ''No capabilities'' {||} else let compl_batches = \<lambda>p t. map (de1 (os\<lparr>nfron := False\<rparr>) \<circ> fst) (filter (\<lambda>(d, t'). t' = t \<and> t \<in> set (filter (\<lambda>t. \<not> frontier_less_equal (front os p) t) (ocaps os p))) (input (os\<lparr>nfron := False\<rparr>) p)); ts = \<lambda>p. rmdups {} (map snd (filter (\<lambda>(d, t). t \<in> set (filter (\<lambda>t. \<not> frontier_less_equal (front os p) t) (ocaps os p))) (input (os\<lparr>nfron := False\<rparr>) p))); osa = os\<lparr>nfron := False, input := \<lambda>p. filter (\<lambda>(d, t). t \<notin> set (filter (\<lambda>t. \<not> frontier_less_equal (front os p) t) (ocaps os p))) (input (os\<lparr>nfron := False\<rparr>) p)\<rparr> in Let {|(concat (map (\<lambda>t. map (\<lambda>x. (x, Cap t 1)) (f (compl_batches 1 t))) (ts 1)), map (\<lambda>t. Cap t 1) (filter (\<lambda>t. \<not> frontier_less_equal (front os 1) t) (ocaps os 1)))|} ((|`|) (\<lambda>(outs, drops). trace (STR ''outs: '' + show_nat (length outs) + STR '' , drops: '' + show_nat (length drops)) (drop_caps (produces osa (map (\<lambda>(d, y). (en2 osa d, y)) outs)) drops))) else {||}))))))) op2'"
-        if "Inl 1 \<notin> ran (case_sum ((\<lambda>_. None)::2 \<Rightarrow> (2 + 2 \<times> 1) option) ((case_option None (Some \<circ> Inr) \<circ>\<circ> case_prod) (\<lambda>nid. (\<lambda>p. case if (nid::2) = 0 then Some (0, 1) else None of None \<Rightarrow> None | Some (offset, q) \<Rightarrow> Some (1 + offset, q))::1 \<Rightarrow> (_ \<times> _) option)))"
-          and "\<not> initia bt_state"
-          and "upfro sg 1"
-          and "propagate_all (summ sg) (pt_tr sg) = Some x2"
-        for x2 :: "((2, 1) location, 't) configuration"
-        using that sorry
-      moreover have "\<exists>op2'. (step Tau)\<^sup>*\<^sup>* (set_spec_op (cUn (cUn S SO) SP) D) op2' \<and> ((~) OO \<U> R OO (\<approx>)) (set_op S D (dataflow_op (sg\<lparr>pt_tr := x2, upfro := (upfro sg)(1 := False)\<rparr>) (map_op (case_sum id id) (case_sum id id) (comp_op (case_sum (\<lambda>_. None) ((case_option None (Some \<circ> Inr) \<circ>\<circ> case_prod) (\<lambda>nid p. case if nid = 0 then Some (0, 1) else None of None \<Rightarrow> None | Some (offset, q) \<Rightarrow> Some (1 + offset, q)))) (case_sum (\<lambda>x. []) (\<lambda>x. map Inr (cbufs x))) (map_op (case_option (Inl 0) (\<lambda>p. Inr (0, 1))) (case_option (Inl 0) (\<lambda>p. Inr (0, 1))) (builder_op False {||} {|1|} ip_state (ooo_input_op_logic {|1|}))) (map_op (case_option (Inl 1) (\<lambda>p. Inr (1, 1))) (case_option (Inl 1) (\<lambda>p. Inr (1, 1))) (builder_op True {|1|} {|1|} (bt_state \<lparr>front := frontier \<circ> (\<lambda>p. c_imp x2 (Loc 1 (Trg 1))), nfron := frontier (c_imp x2 (Loc 1 (Trg 1))) \<noteq> front bt_state 1\<rparr>) (\<lambda>os. if nfron os then if filter (\<lambda>t. \<not> frontier_less_equal (front os 1) t) (ocaps os 1) = [] then trace STR ''No capabilities'' {||} else let compl_batches = \<lambda>p t. map (de1 (os\<lparr>nfron := False\<rparr>) \<circ> fst) (filter (\<lambda>(d, t'). t' = t \<and> t \<in> set (filter (\<lambda>t. \<not> frontier_less_equal (front os p) t) (ocaps os p))) (input (os\<lparr>nfron := False\<rparr>) p)); ts = \<lambda>p. rmdups {} (map snd (filter (\<lambda>(d, t). t \<in> set (filter (\<lambda>t. \<not> frontier_less_equal (front os p) t) (ocaps os p))) (input (os\<lparr>nfron := False\<rparr>) p))); osa = os\<lparr>nfron := False, input := \<lambda>p. filter (\<lambda>(d, t). t \<notin> set (filter (\<lambda>t. \<not> frontier_less_equal (front os p) t) (ocaps os p))) (input (os\<lparr>nfron := False\<rparr>) p)\<rparr> in Let {|(concat (map (\<lambda>t. map (\<lambda>x. (x, Cap t 1)) (f (compl_batches 1 t))) (ts 1)), map (\<lambda>t. Cap t 1) (filter (\<lambda>t. \<not> frontier_less_equal (front os 1) t) (ocaps os 1)))|} ((|`|) (\<lambda>(outs, drops). trace (STR ''outs: '' + show_nat (length outs) + STR '' , drops: '' + show_nat (length drops)) (drop_caps (produces osa (map (\<lambda>(d, y). (en2 osa d, y)) outs)) drops))) else {||}))))))) op2'"
-        if "Inl 1 \<notin> ran (case_sum ((\<lambda>_. None)::2 \<Rightarrow> (2 + 2 \<times> 1) option) ((case_option None (Some \<circ> Inr) \<circ>\<circ> case_prod) (\<lambda>nid. (\<lambda>p. case if (nid::2) = 0 then Some (0, 1) else None of None \<Rightarrow> None | Some (offset, q) \<Rightarrow> Some (1 + offset, q))::1 \<Rightarrow> (_ \<times> _) option)))"
-          and "initia bt_state"
-          and "upfro sg 1"
-          and "propagate_all (summ sg) (pt_tr sg) = Some x2"
-        for x2 :: "((2, 1) location, 't) configuration"
-        using that sorry
-      moreover have "\<exists>op2'. (step Tau)\<^sup>*\<^sup>* (set_spec_op (cUn (cUn S SO) SP) D) op2' \<and> ((~) OO \<U> R OO (\<approx>)) (set_op (cinsert ((1, 1), ab, bb) S) D (dataflow_op sg (map_op (case_sum id id) (case_sum id id) (comp_op (case_sum (\<lambda>_. None) ((case_option None (Some \<circ> Inr) \<circ>\<circ> case_prod) (\<lambda>nid p. case if nid = 0 then Some (0, 1) else None of None \<Rightarrow> None | Some (offset, q) \<Rightarrow> Some (1 + offset, q)))) (case_sum (\<lambda>x. []) (\<lambda>x. map Inr (cbufs x))) (map_op (case_option (Inl 0) (\<lambda>p. Inr (0, 1))) (case_option (Inl 0) (\<lambda>p. Inr (0, 1))) (builder_op False {||} {|1|} ip_state (ooo_input_op_logic {|1|}))) (map_op (case_option (Inl 1) (\<lambda>p. Inr (1, 1))) (case_option (Inl 1) (\<lambda>p. Inr (1, 1))) (builder_op True {|1|} {|1|} (bt_state \<lparr>nfron := False, outpu := (outpu bt_state)(1 := xs)\<rparr>) (\<lambda>os. if nfron os then if filter (\<lambda>t. \<not> frontier_less_equal (front os 1) t) (ocaps os 1) = [] then trace STR ''No capabilities'' {||} else let compl_batches = \<lambda>p t. map (de1 (os\<lparr>nfron := False\<rparr>) \<circ> fst) (filter (\<lambda>(d, t'). t' = t \<and> t \<in> set (filter (\<lambda>t. \<not> frontier_less_equal (front os p) t) (ocaps os p))) (input (os\<lparr>nfron := False\<rparr>) p)); ts = \<lambda>p. rmdups {} (map snd (filter (\<lambda>(d, t). t \<in> set (filter (\<lambda>t. \<not> frontier_less_equal (front os p) t) (ocaps os p))) (input (os\<lparr>nfron := False\<rparr>) p))); osa = os\<lparr>nfron := False, input := \<lambda>p. filter (\<lambda>(d, t). t \<notin> set (filter (\<lambda>t. \<not> frontier_less_equal (front os p) t) (ocaps os p))) (input (os\<lparr>nfron := False\<rparr>) p)\<rparr> in Let {|(concat (map (\<lambda>t. map (\<lambda>x. (x, Cap t 1)) (f (compl_batches 1 t))) (ts 1)), map (\<lambda>t. Cap t 1) (filter (\<lambda>t. \<not> frontier_less_equal (front os 1) t) (ocaps os 1)))|} ((|`|) (\<lambda>(outs, drops). trace (STR ''outs: '' + show_nat (length outs) + STR '' , drops: '' + show_nat (length drops)) (drop_caps (produces osa (map (\<lambda>(d, y). (en2 osa d, y)) outs)) drops))) else {||}))))))) op2'"
-        if "initia bt_state"
-          and "outpu bt_state 1 = (ab, bb) # xs"
-        for ab :: "'d1 + 'd2"
-          and bb :: 't
-          and xs :: "(('d1 + 'd2) \<times> 't) buf"
-        using that sorry
-      ultimately show ?thesis
-        apply -
-        unfolding R_def[symmetric]
-        subgoal premises prems2
-          apply (simp add: wsim_def dataflow_tree_to_operator_def batch_op_def batch_op_logic_def ooo_input_op_def notifier_op_def)
-          apply (intro allI conjI impI)
-          apply (elim step_builder_op_elim step_set_op_elim step_map_op_elim step_comp_op_elim step_dataflow_op_elim conjE ; 
-              clarsimp simp only: IO.simps ; hypsubst_thin ? ; clarsimp simp flip: cin.rep_eq split: option.splits sum.splits prod.splits if_splits ; hypsubst_thin?)
+        apply (simp only: trace_simp)
+        apply (intro allI conjI impI)
+        apply (elim step_builder_op_elim step_set_op_elim step_map_op_elim step_comp_op_elim step_dataflow_op_elim conjE ; 
+            clarsimp simp only: IO.simps ; hypsubst_thin ? ; clarsimp simp flip: cin.rep_eq split: option.splits sum.splits prod.splits if_splits ; hypsubst_thin?)
+        subgoal 
+          apply -
+          apply (intro exI conjI relcomppI)
+             apply (rule step_set_spec_op_intro_Out)
+                apply (rule refl)
+               apply simp
+              apply simp
+             apply (rule refl)
+            apply (rule bisim_refl)
+           defer
+           apply (rule wbisim_refl)
+          apply (rule wb_upto_b_base)
+          unfolding R_def[simplified]
+          apply (intro exI conjI)
+          unfolding wsim_def dataflow_tree_to_operator_def batch_op_def batch_op_logic_def ooo_input_op_def ooo_input_op_logic_def notifier_op_def
+                 apply simp
+                 apply (simp only: trace_simp)
+                 apply (simp add: SIM1)
+                apply (simp add: SIM1)
+               apply (simp add: SIM1)
+              apply (simp add: SIM1)
           subgoal
-            using prems2(1) by assumption
-          subgoal
-            using prems2(2) by assumption
-          subgoal
-            using prems2(3) by assumption
-          subgoal
-            using prems2(4) by assumption
-          subgoal
-            using prems2(5) by assumption
-          subgoal
-            using prems2(6) by assumption
-          subgoal
-            using prems2(7) by assumption
-          subgoal
-            using prems2(8) by assumption
-          subgoal
-            using prems2(9) by assumption
-          subgoal
-            using prems2(10) by assumption
-          subgoal
-            using prems2(11) by assumption
+            using SIM1
+            by (auto simp add: all_isl_def Src_from_Trg_def my_summ_def BULK_BENQ_def outputs_at_target_def split: prod.splits)
+          using SIM1 apply fastforce+
           done
+                 defer
+        defer
+        subgoal for d t
+      apply (cases "cbufs (1, 1)"; simp add: BHD_def BTL_def)
+      subgoal for a as
+          apply (intro exI conjI relcomppI)
+          apply (rule rtranclp.intros(1))
+            apply (rule bisim_refl)
+          defer
+           apply (rule wbisim_refl)
+          apply (rule wb_upto_b_base)
+        unfolding R_def[simplified]
+          apply (rule exI[of _ "os(1 := consumes (os 1) 1 t d)"])
+          apply (rule exI[of _ sg])
+          apply (rule exI[of _ "BTL (1, 1) cbufs"])
+          apply (rule exI[of _ inps])
+          apply (rule exI[of _ S])
+          apply (rule exI[of _ D])
+          apply (intro conjI)
+  unfolding dataflow_tree_to_operator_def batch_op_def batch_op_logic_def ooo_input_op_def ooo_input_op_logic_def notifier_op_def
+                 apply simp
+                 apply (simp only: trace_simp)
+         apply (simp add: SIM1 BTL_def BENQ_def add_caps_def operator_state.defs(3))
+         apply (rule arg_cong3[where f=set_op])
+           apply (rule refl)+
+            apply (rule arg_cong2[where f=dataflow_op])
+           apply (rule refl)+
+            apply (rule arg_cong3[where f=map_op])
+           apply (rule refl)+
+            apply (rule arg_cong4[where f=comp_op])
+            apply (rule refl)+
+            apply (rule arg_cong2[where f=case_sum])
+          apply (rule refl)+
+  apply fastforce
+            apply (rule arg_cong3[where f=map_op])
+              apply (rule refl)+
+            apply (rule arg_cong3[where f=map_op])
+              apply (rule refl)+
+            apply (rule arg_cong5[where f=builder_op])
+           apply (rule refl)+
+        apply (simp add: consumes_def add_caps_def  enum_num1_def operator_state.defs(3))
+           apply (rule refl)+
+  subgoal premises prems2
+    apply (rule arg_cong2[where f=set_spec_op])
+     apply simp_all
+    using SIM1(6,8,9) apply -
+    apply (simp only: cUn_assoc)
+    apply (rule arg_cong2[where f= cUn])
+     apply simp_all
+    subgoal premises
+      apply (rule arg_cong2[where f= cUn])
+       apply simp_all
+      unfolding inputs_at_target_def 
+      apply simp
+      apply (rule arg_cong2[where f= cUn])
+      subgoal
+        apply (rule arg_cong[where f= cUnion])
+        apply (rule arg_cong2[where f=cimage])
+         apply simp_all
+        apply (rule ext)+
+        apply (rule arg_cong[where f=cset_of_llist])
+        apply (rule arg_cong[where f=llist_of])
+        apply (rule map_cong)
+         apply simp_all
+        apply (rule arg_cong[where f=f])
+        apply (rule arg_cong[where f=list_of])
+        apply (rule arg_cong2[where f=lshift])
+         apply simp_all
+        apply (rule map_cong)
+         apply simp_all
+        apply (rule filter_cong)
+         apply simp_all
+        apply (rule map_cong)
+         apply simp_all
+        apply (simp flip: BULK_BENQ_assoc)
+        unfolding consumes_def add_caps_def BULK_BENQ_def BTL_def
+        apply simp
         done
-    qed
-  qed
+      subgoal
+        apply (rule arg_cong[where f= cUnion])
+        apply (rule arg_cong2[where f=cimage])
+         apply (rule ext)+
+         apply (rule arg_cong[where f=cset_of_llist])
+         apply (rule arg_cong[where f=llist_of])
+         apply (rule map_cong)
+          apply simp_all
+         apply (rule arg_cong[where f=f])
+         apply (rule arg_cong[where f=list_of])
+         apply (rule arg_cong2[where f=lshift])
+          apply simp_all
+         apply (rule map_cong)
+          apply simp_all
+         apply (rule filter_cong)
+          apply simp_all
+         apply (rule map_cong)
+          apply simp_all
+         apply (simp flip: BULK_BENQ_assoc)
+        unfolding consumes_def add_caps_def BULK_BENQ_def BTL_def
+         apply simp
+        unfolding consumes_def add_caps_def BULK_BENQ_def BTL_def
+        apply simp
+        done
+      done
+    done
+
+        find_theorems BULK_BENQ name: ass
+
+end
+  using SIM1(1,12,13,14) apply -
+  apply simp
+  apply hypsubst_thin
+
+
+  find_theorems c
+
+  defer
+  defer
+  defer
+  defer
+  defer
+  defer
+
+
+  apply (simp_all only: SIM1 dataflow_tree_to_graph_to_my_summ)
+  defer
+  using SIM1(21) apply simp
+  using SIM1(1,20) apply simp
+  defer
+  defer
+  defer
+  using SIM1(1,16) apply simp
+  using SIM1(1,15) apply simp
+  using SIM1(22) apply simp
+
+  find_theorems graph_to_edges
+
+end
+
+  apply (rule arg_cong[where f="cUnion"])
+  apply (rule arg_cong2[where f="cimage"])
+  apply (rule ext)+
+  apply (simp split: prod.splits)
+  apply (rule refl)
+
+
+
+end
+  moreover have "\<exists>op2'. (step Tau)\<^sup>*\<^sup>* (set_spec_op (cUn (cUn S SO) SP) D) op2' \<and> ((~) OO \<U> R OO (\<approx>)) (set_op S D (dataflow_op sg (map_op (case_sum id id) (case_sum id id) (comp_op (case_sum (\<lambda>_. None) ((case_option None (Some \<circ> Inr) \<circ>\<circ> case_prod) (\<lambda>nid p. case if nid = 0 then Some (0, 1) else None of None \<Rightarrow> None | Some (offset, q) \<Rightarrow> Some (1 + offset, q)))) (case_sum (\<lambda>x. []) (BENQ (1, 1) (Inr (a, b)) (\<lambda>x. map Inr (cbufs x)))) (map_op (case_option (Inl 0) (\<lambda>p. Inr (0, 1))) (case_option (Inl 0) (\<lambda>p. Inr (0, 1))) (builder_op False {||} {|1|} (ip_state\<lparr>outpu := (outpu ip_state)(1 := xs)\<rparr>) (ooo_input_op_logic {|1|}))) (map_op (case_option (Inl 1) (\<lambda>p. Inr (1, 1))) (case_option (Inl 1) (\<lambda>p. Inr (1, 1))) (builder_op True {|1|} {|1|} (bt_state\<lparr>nfron := False\<rparr>) (\<lambda>os. if nfron os then if filter (\<lambda>t. \<not> frontier_less_equal (front os 1) t) (ocaps os 1) = [] then trace STR ''No capabilities'' {||} else let compl_batches = \<lambda>p t. map (de1 (os\<lparr>nfron := False\<rparr>) \<circ> fst) (filter (\<lambda>(d, t'). t' = t \<and> t \<in> set (filter (\<lambda>t. \<not> frontier_less_equal (front os p) t) (ocaps os p))) (input (os\<lparr>nfron := False\<rparr>) p)); ts = \<lambda>p. rmdups {} (map snd (filter (\<lambda>(d, t). t \<in> set (filter (\<lambda>t. \<not> frontier_less_equal (front os p) t) (ocaps os p))) (input (os\<lparr>nfron := False\<rparr>) p))); osa = os\<lparr>nfron := False, input := \<lambda>p. filter (\<lambda>(d, t). t \<notin> set (filter (\<lambda>t. \<not> frontier_less_equal (front os p) t) (ocaps os p))) (input (os\<lparr>nfron := False\<rparr>) p)\<rparr> in Let {|(concat (map (\<lambda>t. map (\<lambda>x. (x, Cap t 1)) (f (compl_batches 1 t))) (ts 1)), map (\<lambda>t. Cap t 1) (filter (\<lambda>t. \<not> frontier_less_equal (front os 1) t) (ocaps os 1)))|} ((|`|) (\<lambda>(outs, drops). trace (STR ''outs: '' + show_nat (length outs) + STR '' , drops: '' + show_nat (length drops)) (drop_caps (produces osa (map (\<lambda>(d, y). (en2 osa d, y)) outs)) drops))) else {||}))))))) op2'"
+    if "initia ip_state"
+      and "outpu ip_state 1 = (a, b) # xs"
+    for a :: "'d1 + 'd2"
+      and b :: 't
+      and xs :: "(('d1 + 'd2) \<times> 't) buf"
+    using that sorry
+  moreover have "\<exists>op2'. (step Tau)\<^sup>*\<^sup>* (set_spec_op (cUn (cUn S SO) SP) D) op2' \<and> ((~) OO \<U> R OO (\<approx>)) (set_op S D (dataflow_op sg (map_op (case_sum id id) (case_sum id id) (comp_op (case_sum (\<lambda>_. None) ((case_option None (Some \<circ> Inr) \<circ>\<circ> case_prod) (\<lambda>nid p. case if nid = 0 then Some (0, 1) else None of None \<Rightarrow> None | Some (offset, q) \<Rightarrow> Some (1 + offset, q)))) (case_sum (\<lambda>x. []) (BTL (1, 1) (\<lambda>x. map Inr (cbufs x)))) (map_op (case_option (Inl 0) (\<lambda>p. Inr (0, 1))) (case_option (Inl 0) (\<lambda>p. Inr (0, 1))) (builder_op False {||} {|1|} ip_state (ooo_input_op_logic {|1|}))) \<oslash>)))) op2'"
+    if "Inr (1, 1) \<in> ran (case_sum ((\<lambda>_. None)::2 \<Rightarrow> (2 + 2 \<times> 1) option) ((case_option None (Some \<circ> Inr) \<circ>\<circ> case_prod) (\<lambda>nid. (\<lambda>p. case if (nid::2) = 0 then Some (0, 1) else None of None \<Rightarrow> None | Some (offset, q) \<Rightarrow> Some (1 + offset, q))::1 \<Rightarrow> (_ \<times> _) option)))"
+      and "cbufs (1, 1) \<noteq> []"
+      and "initia bt_state"
+      and "is_Inl (BHD (1, 1) (\<lambda>x. map Inr (cbufs x))::((1, 't) shared_state + (1 \<Rightarrow> 't antichain)) + ('d1 + 'd2) \<times> 't)"
+    using that sorry
+  moreover have "\<exists>op2'. (step Tau)\<^sup>*\<^sup>* (set_spec_op (cUn (cUn S SO) SP) D) op2' \<and> ((~) OO \<U> R OO (\<approx>)) (set_op S D (dataflow_op sg (map_op (case_sum id id) (case_sum id id) (comp_op (case_sum (\<lambda>_. None) ((case_option None (Some \<circ> Inr) \<circ>\<circ> case_prod) (\<lambda>nid p. case if nid = 0 then Some (0, 1) else None of None \<Rightarrow> None | Some (offset, q) \<Rightarrow> Some (1 + offset, q)))) (case_sum (\<lambda>x. []) (BTL (1, 1) (\<lambda>x. map Inr (cbufs x)))) (map_op (case_option (Inl 0) (\<lambda>p. Inr (0, 1))) (case_option (Inl 0) (\<lambda>p. Inr (0, 1))) (builder_op False {||} {|1|} ip_state (ooo_input_op_logic {|1|}))) (map_op (case_option (Inl 1) (\<lambda>p. Inr (1, 1))) (case_option (Inl 1) (\<lambda>p. Inr (1, 1))) (builder_op True {|1|} {|1|} (consumes (bt_state\<lparr>nfron := False\<rparr>) 1 t d) (\<lambda>os. if nfron os then if filter (\<lambda>t. \<not> frontier_less_equal (front os 1) t) (ocaps os 1) = [] then trace STR ''No capabilities'' {||} else let compl_batches = \<lambda>p t. map (de1 (os\<lparr>nfron := False\<rparr>) \<circ> fst) (filter (\<lambda>(d, t'). t' = t \<and> t \<in> set (filter (\<lambda>t. \<not> frontier_less_equal (front os p) t) (ocaps os p))) (input (os\<lparr>nfron := False\<rparr>) p)); ts = \<lambda>p. rmdups {} (map snd (filter (\<lambda>(d, t). t \<in> set (filter (\<lambda>t. \<not> frontier_less_equal (front os p) t) (ocaps os p))) (input (os\<lparr>nfron := False\<rparr>) p))); osa = os\<lparr>nfron := False, input := \<lambda>p. filter (\<lambda>(d, t). t \<notin> set (filter (\<lambda>t. \<not> frontier_less_equal (front os p) t) (ocaps os p))) (input (os\<lparr>nfron := False\<rparr>) p)\<rparr> in Let {|(concat (map (\<lambda>t. map (\<lambda>x. (x, Cap t 1)) (f (compl_batches 1 t))) (ts 1)), map (\<lambda>t. Cap t 1) (filter (\<lambda>t. \<not> frontier_less_equal (front os 1) t) (ocaps os 1)))|} ((|`|) (\<lambda>(outs, drops). trace (STR ''outs: '' + show_nat (length outs) + STR '' , drops: '' + show_nat (length drops)) (drop_caps (produces osa (map (\<lambda>(d, y). (en2 osa d, y)) outs)) drops))) else {||}))))))) op2'"
+    if "Inr (1, 1) \<in> ran (case_sum ((\<lambda>_. None)::2 \<Rightarrow> (2 + 2 \<times> 1) option) ((case_option None (Some \<circ> Inr) \<circ>\<circ> case_prod) (\<lambda>nid. (\<lambda>p. case if (nid::2) = 0 then Some (0, 1) else None of None \<Rightarrow> None | Some (offset, q) \<Rightarrow> Some (1 + offset, q))::1 \<Rightarrow> (_ \<times> _) option)))"
+      and "cbufs (1, 1) \<noteq> []"
+      and "initia bt_state"
+      and "(Inr (d, t)::((1, 't) shared_state + (1 \<Rightarrow> 't antichain)) + ('d1 + 'd2) \<times> 't) = BHD (1, 1) (\<lambda>x. map Inr (cbufs x))"
+    for d :: "'d1 + 'd2"
+      and t :: 't
+    using that sorry
+  moreover have "\<exists>op2'. (step Tau)\<^sup>*\<^sup>* (set_spec_op (cUn (cUn S SO) SP) D) op2' \<and> ((~) OO \<U> R OO (\<approx>)) (set_op S D (dataflow_op sg (map_op (case_sum id id) (case_sum id id) (comp_op (case_sum (\<lambda>_. None) ((case_option None (Some \<circ> Inr) \<circ>\<circ> case_prod) (\<lambda>nid p. case if nid = 0 then Some (0, 1) else None of None \<Rightarrow> None | Some (offset, q) \<Rightarrow> Some (1 + offset, q)))) (case_sum (\<lambda>x. []) (\<lambda>x. map Inr (cbufs x))) (map_op (case_option (Inl 0) (\<lambda>p. Inr (0, 1))) (case_option (Inl 0) (\<lambda>p. Inr (0, 1))) (builder_op False {||} {|1|} os' (ooo_input_op_logic {|1|}))) (map_op (case_option (Inl 1) (\<lambda>p. Inr (1, 1))) (case_option (Inl 1) (\<lambda>p. Inr (1, 1))) (builder_op True {|1|} {|1|} (bt_state\<lparr>nfron := False\<rparr>) (\<lambda>os. if nfron os then if filter (\<lambda>t. \<not> frontier_less_equal (front os 1) t) (ocaps os 1) = [] then trace STR ''No capabilities'' {||} else let compl_batches = \<lambda>p t. map (de1 (os\<lparr>nfron := False\<rparr>) \<circ> fst) (filter (\<lambda>(d, t'). t' = t \<and> t \<in> set (filter (\<lambda>t. \<not> frontier_less_equal (front os p) t) (ocaps os p))) (input (os\<lparr>nfron := False\<rparr>) p)); ts = \<lambda>p. rmdups {} (map snd (filter (\<lambda>(d, t). t \<in> set (filter (\<lambda>t. \<not> frontier_less_equal (front os p) t) (ocaps os p))) (input (os\<lparr>nfron := False\<rparr>) p))); osa = os\<lparr>nfron := False, input := \<lambda>p. filter (\<lambda>(d, t). t \<notin> set (filter (\<lambda>t. \<not> frontier_less_equal (front os p) t) (ocaps os p))) (input (os\<lparr>nfron := False\<rparr>) p)\<rparr> in Let {|(concat (map (\<lambda>t. map (\<lambda>x. (x, Cap t 1)) (f (compl_batches 1 t))) (ts 1)), map (\<lambda>t. Cap t 1) (filter (\<lambda>t. \<not> frontier_less_equal (front os 1) t) (ocaps os 1)))|} ((|`|) (\<lambda>(outs, drops). trace (STR ''outs: '' + show_nat (length outs) + STR '' , drops: '' + show_nat (length drops)) (drop_caps (produces osa (map (\<lambda>(d, y). (en2 osa d, y)) outs)) drops))) else {||}))))))) op2'"
+    if "initia ip_state"
+      and "os' |\<in>| ooo_input_op_logic {|1|} ip_state"
+      and "ocaps ip_state 1 \<noteq> []"
+    for os' :: "(1, 'd1 + 'd2, 'd1, 't) input_state"
+    using that sorry
+  moreover have "\<exists>op2'. (step Tau)\<^sup>*\<^sup>* (set_spec_op (cUn (cUn S SO) SP) D) op2' \<and> ((~) OO \<U> R OO (\<approx>)) (set_op S D (dataflow_op (sg\<lparr>upfro := \<lambda>_. True, pt_tr := change_multiplicities (summ sg) (extract_progress 1 (edges sg) st) (pt_tr sg)\<rparr>) (map_op (case_sum id id) (case_sum id id) (comp_op (case_sum (\<lambda>_. None) ((case_option None (Some \<circ> Inr) \<circ>\<circ> case_prod) (\<lambda>nid p. case if nid = 0 then Some (0, 1) else None of None \<Rightarrow> None | Some (offset, q) \<Rightarrow> Some (1 + offset, q)))) (case_sum (\<lambda>x. []) (\<lambda>x. map Inr (cbufs x))) (map_op (case_option (Inl 0) (\<lambda>p. Inr (0, 1))) (case_option (Inl 0) (\<lambda>p. Inr (0, 1))) (builder_op False {||} {|1|} ip_state (ooo_input_op_logic {|1|}))) (map_op (case_option (Inl 1) (\<lambda>p. Inr (1, 1))) (case_option (Inl 1) (\<lambda>p. Inr (1, 1))) (builder_op True {|1|} {|1|} os' (\<lambda>os. if nfron os then if filter (\<lambda>t. \<not> frontier_less_equal (front os 1) t) (ocaps os 1) = [] then trace STR ''No capabilities'' {||} else let compl_batches = \<lambda>p t. map (de1 (os\<lparr>nfron := False\<rparr>) \<circ> fst) (filter (\<lambda>(d, t'). t' = t \<and> t \<in> set (filter (\<lambda>t. \<not> frontier_less_equal (front os p) t) (ocaps os p))) (input (os\<lparr>nfron := False\<rparr>) p)); ts = \<lambda>p. rmdups {} (map snd (filter (\<lambda>(d, t). t \<in> set (filter (\<lambda>t. \<not> frontier_less_equal (front os p) t) (ocaps os p))) (input (os\<lparr>nfron := False\<rparr>) p))); osa = os\<lparr>nfron := False, input := \<lambda>p. filter (\<lambda>(d, t). t \<notin> set (filter (\<lambda>t. \<not> frontier_less_equal (front os p) t) (ocaps os p))) (input (os\<lparr>nfron := False\<rparr>) p)\<rparr> in Let {|(concat (map (\<lambda>t. map (\<lambda>x. (x, Cap t 1)) (f (compl_batches 1 t))) (ts 1)), map (\<lambda>t. Cap t 1) (filter (\<lambda>t. \<not> frontier_less_equal (front os 1) t) (ocaps os 1)))|} ((|`|) (\<lambda>(outs, drops). trace (STR ''outs: '' + show_nat (length outs) + STR '' , drops: '' + show_nat (length drops)) (drop_caps (produces osa (map (\<lambda>(d, y). (en2 osa d, y)) outs)) drops))) else {||}))))))) op2'"
+    if "initia bt_state"
+      and "has_progress (bt_state\<lparr>nfron := False\<rparr>)"
+      and "(os', st) = obtain_progress (bt_state\<lparr>nfron := False\<rparr>)"
+    for st :: "(1, 't) shared_state"
+      and os' :: "(1, 'd1 + 'd2, 'd1, 'd2, 't) operator_state_ty2"
+    using that sorry
+  moreover have "\<exists>op2'. (step Tau)\<^sup>*\<^sup>* (set_spec_op (cUn (cUn S SO) SP) D) op2' \<and> ((~) OO \<U> R OO (\<approx>)) (set_op S D (dataflow_op (sg\<lparr>upfro := \<lambda>_. True, pt_tr := change_multiplicities (summ sg) (extract_progress 0 (edges sg) st) (pt_tr sg)\<rparr>) (map_op (case_sum id id) (case_sum id id) (comp_op (case_sum (\<lambda>_. None) ((case_option None (Some \<circ> Inr) \<circ>\<circ> case_prod) (\<lambda>nid p. case if nid = 0 then Some (0, 1) else None of None \<Rightarrow> None | Some (offset, q) \<Rightarrow> Some (1 + offset, q)))) (case_sum (\<lambda>x. []) (\<lambda>x. map Inr (cbufs x))) (map_op (case_option (Inl 0) (\<lambda>p. Inr (0, 1))) (case_option (Inl 0) (\<lambda>p. Inr (0, 1))) (builder_op False {||} {|1|} os' (ooo_input_op_logic {|1|}))) (map_op (case_option (Inl 1) (\<lambda>p. Inr (1, 1))) (case_option (Inl 1) (\<lambda>p. Inr (1, 1))) (builder_op True {|1|} {|1|} (bt_state\<lparr>nfron := False\<rparr>) (\<lambda>os. if nfron os then if filter (\<lambda>t. \<not> frontier_less_equal (front os 1) t) (ocaps os 1) = [] then trace STR ''No capabilities'' {||} else let compl_batches = \<lambda>p t. map (de1 (os\<lparr>nfron := False\<rparr>) \<circ> fst) (filter (\<lambda>(d, t'). t' = t \<and> t \<in> set (filter (\<lambda>t. \<not> frontier_less_equal (front os p) t) (ocaps os p))) (input (os\<lparr>nfron := False\<rparr>) p)); ts = \<lambda>p. rmdups {} (map snd (filter (\<lambda>(d, t). t \<in> set (filter (\<lambda>t. \<not> frontier_less_equal (front os p) t) (ocaps os p))) (input (os\<lparr>nfron := False\<rparr>) p))); osa = os\<lparr>nfron := False, input := \<lambda>p. filter (\<lambda>(d, t). t \<notin> set (filter (\<lambda>t. \<not> frontier_less_equal (front os p) t) (ocaps os p))) (input (os\<lparr>nfron := False\<rparr>) p)\<rparr> in Let {|(concat (map (\<lambda>t. map (\<lambda>x. (x, Cap t 1)) (f (compl_batches 1 t))) (ts 1)), map (\<lambda>t. Cap t 1) (filter (\<lambda>t. \<not> frontier_less_equal (front os 1) t) (ocaps os 1)))|} ((|`|) (\<lambda>(outs, drops). trace (STR ''outs: '' + show_nat (length outs) + STR '' , drops: '' + show_nat (length drops)) (drop_caps (produces osa (map (\<lambda>(d, y). (en2 osa d, y)) outs)) drops))) else {||}))))))) op2'"
+    if "initia ip_state"
+      and "has_progress ip_state"
+      and "(os', st) = obtain_progress ip_state"
+    for st :: "(1, 't) shared_state"
+      and os' :: "(1, 'd1 + 'd2, 'd1, 't) input_state"
+    using that sorry
+  moreover have "\<exists>op2'. (step Tau)\<^sup>*\<^sup>* (set_spec_op (cUn (cUn S SO) SP) D) op2' \<and> ((~) OO \<U> R OO (\<approx>)) (set_op S D (dataflow_op (sg\<lparr>pt_tr := x2, upfro := (upfro sg)(0 := False)\<rparr>) (map_op (case_sum id id) (case_sum id id) (comp_op (case_sum (\<lambda>_. None) ((case_option None (Some \<circ> Inr) \<circ>\<circ> case_prod) (\<lambda>nid p. case if nid = 0 then Some (0, 1) else None of None \<Rightarrow> None | Some (offset, q) \<Rightarrow> Some (1 + offset, q)))) (case_sum (\<lambda>x. []) (\<lambda>x. map Inr (cbufs x))) (map_op (case_option (Inl 0) (\<lambda>p. Inr (0, 1))) (case_option (Inl 0) (\<lambda>p. Inr (0, 1))) (builder_op False {||} {|1|} (ip_state \<lparr>front := frontier \<circ> (\<lambda>p. c_imp x2 (Loc 0 (Trg 1))), initia := True, nfron := True\<rparr>) (ooo_input_op_logic {|1|}))) (map_op (case_option (Inl 1) (\<lambda>p. Inr (1, 1))) (case_option (Inl 1) (\<lambda>p. Inr (1, 1))) (builder_op True {|1|} {|1|} (bt_state\<lparr>nfron := False\<rparr>) (\<lambda>os. if nfron os then if filter (\<lambda>t. \<not> frontier_less_equal (front os 1) t) (ocaps os 1) = [] then trace STR ''No capabilities'' {||} else let compl_batches = \<lambda>p t. map (de1 (os\<lparr>nfron := False\<rparr>) \<circ> fst) (filter (\<lambda>(d, t'). t' = t \<and> t \<in> set (filter (\<lambda>t. \<not> frontier_less_equal (front os p) t) (ocaps os p))) (input (os\<lparr>nfron := False\<rparr>) p)); ts = \<lambda>p. rmdups {} (map snd (filter (\<lambda>(d, t). t \<in> set (filter (\<lambda>t. \<not> frontier_less_equal (front os p) t) (ocaps os p))) (input (os\<lparr>nfron := False\<rparr>) p))); osa = os\<lparr>nfron := False, input := \<lambda>p. filter (\<lambda>(d, t). t \<notin> set (filter (\<lambda>t. \<not> frontier_less_equal (front os p) t) (ocaps os p))) (input (os\<lparr>nfron := False\<rparr>) p)\<rparr> in Let {|(concat (map (\<lambda>t. map (\<lambda>x. (x, Cap t 1)) (f (compl_batches 1 t))) (ts 1)), map (\<lambda>t. Cap t 1) (filter (\<lambda>t. \<not> frontier_less_equal (front os 1) t) (ocaps os 1)))|} ((|`|) (\<lambda>(outs, drops). trace (STR ''outs: '' + show_nat (length outs) + STR '' , drops: '' + show_nat (length drops)) (drop_caps (produces osa (map (\<lambda>(d, y). (en2 osa d, y)) outs)) drops))) else {||}))))))) op2'"
+    if "upfro sg 0"
+      and "\<not> initia ip_state"
+      and "propagate_all (summ sg) (pt_tr sg) = Some x2"
+    for x2 :: "((2, 1) location, 't) configuration"
+    using that sorry
+  moreover have "\<exists>op2'. (step Tau)\<^sup>*\<^sup>* (set_spec_op (cUn (cUn S SO) SP) D) op2' \<and> ((~) OO \<U> R OO (\<approx>)) (set_op S D (dataflow_op (sg\<lparr>pt_tr := x2, upfro := (upfro sg)(1 := False)\<rparr>) (map_op (case_sum id id) (case_sum id id) (comp_op (case_sum (\<lambda>_. None) ((case_option None (Some \<circ> Inr) \<circ>\<circ> case_prod) (\<lambda>nid p. case if nid = 0 then Some (0, 1) else None of None \<Rightarrow> None | Some (offset, q) \<Rightarrow> Some (1 + offset, q)))) (case_sum (\<lambda>x. []) (\<lambda>x. map Inr (cbufs x))) (map_op (case_option (Inl 0) (\<lambda>p. Inr (0, 1))) (case_option (Inl 0) (\<lambda>p. Inr (0, 1))) (builder_op False {||} {|1|} ip_state (ooo_input_op_logic {|1|}))) (map_op (case_option (Inl 1) (\<lambda>p. Inr (1, 1))) (case_option (Inl 1) (\<lambda>p. Inr (1, 1))) (builder_op True {|1|} {|1|} (bt_state \<lparr>front := frontier \<circ> (\<lambda>p. c_imp x2 (Loc 1 (Trg 1))), initia := True, nfron := True\<rparr>) (\<lambda>os. if nfron os then if filter (\<lambda>t. \<not> frontier_less_equal (front os 1) t) (ocaps os 1) = [] then trace STR ''No capabilities'' {||} else let compl_batches = \<lambda>p t. map (de1 (os\<lparr>nfron := False\<rparr>) \<circ> fst) (filter (\<lambda>(d, t'). t' = t \<and> t \<in> set (filter (\<lambda>t. \<not> frontier_less_equal (front os p) t) (ocaps os p))) (input (os\<lparr>nfron := False\<rparr>) p)); ts = \<lambda>p. rmdups {} (map snd (filter (\<lambda>(d, t). t \<in> set (filter (\<lambda>t. \<not> frontier_less_equal (front os p) t) (ocaps os p))) (input (os\<lparr>nfron := False\<rparr>) p))); osa = os\<lparr>nfron := False, input := \<lambda>p. filter (\<lambda>(d, t). t \<notin> set (filter (\<lambda>t. \<not> frontier_less_equal (front os p) t) (ocaps os p))) (input (os\<lparr>nfron := False\<rparr>) p)\<rparr> in Let {|(concat (map (\<lambda>t. map (\<lambda>x. (x, Cap t 1)) (f (compl_batches 1 t))) (ts 1)), map (\<lambda>t. Cap t 1) (filter (\<lambda>t. \<not> frontier_less_equal (front os 1) t) (ocaps os 1)))|} ((|`|) (\<lambda>(outs, drops). trace (STR ''outs: '' + show_nat (length outs) + STR '' , drops: '' + show_nat (length drops)) (drop_caps (produces osa (map (\<lambda>(d, y). (en2 osa d, y)) outs)) drops))) else {||}))))))) op2'"
+    if "Inl 1 \<notin> ran (case_sum ((\<lambda>_. None)::2 \<Rightarrow> (2 + 2 \<times> 1) option) ((case_option None (Some \<circ> Inr) \<circ>\<circ> case_prod) (\<lambda>nid. (\<lambda>p. case if (nid::2) = 0 then Some (0, 1) else None of None \<Rightarrow> None | Some (offset, q) \<Rightarrow> Some (1 + offset, q))::1 \<Rightarrow> (_ \<times> _) option)))"
+      and "\<not> initia bt_state"
+      and "upfro sg 1"
+      and "propagate_all (summ sg) (pt_tr sg) = Some x2"
+    for x2 :: "((2, 1) location, 't) configuration"
+    using that sorry
+  moreover have "\<exists>op2'. (step Tau)\<^sup>*\<^sup>* (set_spec_op (cUn (cUn S SO) SP) D) op2' \<and> ((~) OO \<U> R OO (\<approx>)) (set_op S D (dataflow_op (sg\<lparr>pt_tr := x2, upfro := (upfro sg)(1 := False)\<rparr>) (map_op (case_sum id id) (case_sum id id) (comp_op (case_sum (\<lambda>_. None) ((case_option None (Some \<circ> Inr) \<circ>\<circ> case_prod) (\<lambda>nid p. case if nid = 0 then Some (0, 1) else None of None \<Rightarrow> None | Some (offset, q) \<Rightarrow> Some (1 + offset, q)))) (case_sum (\<lambda>x. []) (\<lambda>x. map Inr (cbufs x))) (map_op (case_option (Inl 0) (\<lambda>p. Inr (0, 1))) (case_option (Inl 0) (\<lambda>p. Inr (0, 1))) (builder_op False {||} {|1|} ip_state (ooo_input_op_logic {|1|}))) (map_op (case_option (Inl 1) (\<lambda>p. Inr (1, 1))) (case_option (Inl 1) (\<lambda>p. Inr (1, 1))) (builder_op True {|1|} {|1|} (bt_state \<lparr>front := frontier \<circ> (\<lambda>p. c_imp x2 (Loc 1 (Trg 1))), nfron := frontier (c_imp x2 (Loc 1 (Trg 1))) \<noteq> front bt_state 1\<rparr>) (\<lambda>os. if nfron os then if filter (\<lambda>t. \<not> frontier_less_equal (front os 1) t) (ocaps os 1) = [] then trace STR ''No capabilities'' {||} else let compl_batches = \<lambda>p t. map (de1 (os\<lparr>nfron := False\<rparr>) \<circ> fst) (filter (\<lambda>(d, t'). t' = t \<and> t \<in> set (filter (\<lambda>t. \<not> frontier_less_equal (front os p) t) (ocaps os p))) (input (os\<lparr>nfron := False\<rparr>) p)); ts = \<lambda>p. rmdups {} (map snd (filter (\<lambda>(d, t). t \<in> set (filter (\<lambda>t. \<not> frontier_less_equal (front os p) t) (ocaps os p))) (input (os\<lparr>nfron := False\<rparr>) p))); osa = os\<lparr>nfron := False, input := \<lambda>p. filter (\<lambda>(d, t). t \<notin> set (filter (\<lambda>t. \<not> frontier_less_equal (front os p) t) (ocaps os p))) (input (os\<lparr>nfron := False\<rparr>) p)\<rparr> in Let {|(concat (map (\<lambda>t. map (\<lambda>x. (x, Cap t 1)) (f (compl_batches 1 t))) (ts 1)), map (\<lambda>t. Cap t 1) (filter (\<lambda>t. \<not> frontier_less_equal (front os 1) t) (ocaps os 1)))|} ((|`|) (\<lambda>(outs, drops). trace (STR ''outs: '' + show_nat (length outs) + STR '' , drops: '' + show_nat (length drops)) (drop_caps (produces osa (map (\<lambda>(d, y). (en2 osa d, y)) outs)) drops))) else {||}))))))) op2'"
+    if "Inl 1 \<notin> ran (case_sum ((\<lambda>_. None)::2 \<Rightarrow> (2 + 2 \<times> 1) option) ((case_option None (Some \<circ> Inr) \<circ>\<circ> case_prod) (\<lambda>nid. (\<lambda>p. case if (nid::2) = 0 then Some (0, 1) else None of None \<Rightarrow> None | Some (offset, q) \<Rightarrow> Some (1 + offset, q))::1 \<Rightarrow> (_ \<times> _) option)))"
+      and "initia bt_state"
+      and "upfro sg 1"
+      and "propagate_all (summ sg) (pt_tr sg) = Some x2"
+    for x2 :: "((2, 1) location, 't) configuration"
+    using that sorry
+  moreover have "\<exists>op2'. (step Tau)\<^sup>*\<^sup>* (set_spec_op (cUn (cUn S SO) SP) D) op2' \<and> ((~) OO \<U> R OO (\<approx>)) (set_op (cinsert ((1, 1), ab, bb) S) D (dataflow_op sg (map_op (case_sum id id) (case_sum id id) (comp_op (case_sum (\<lambda>_. None) ((case_option None (Some \<circ> Inr) \<circ>\<circ> case_prod) (\<lambda>nid p. case if nid = 0 then Some (0, 1) else None of None \<Rightarrow> None | Some (offset, q) \<Rightarrow> Some (1 + offset, q)))) (case_sum (\<lambda>x. []) (\<lambda>x. map Inr (cbufs x))) (map_op (case_option (Inl 0) (\<lambda>p. Inr (0, 1))) (case_option (Inl 0) (\<lambda>p. Inr (0, 1))) (builder_op False {||} {|1|} ip_state (ooo_input_op_logic {|1|}))) (map_op (case_option (Inl 1) (\<lambda>p. Inr (1, 1))) (case_option (Inl 1) (\<lambda>p. Inr (1, 1))) (builder_op True {|1|} {|1|} (bt_state \<lparr>nfron := False, outpu := (outpu bt_state)(1 := xs)\<rparr>) (\<lambda>os. if nfron os then if filter (\<lambda>t. \<not> frontier_less_equal (front os 1) t) (ocaps os 1) = [] then trace STR ''No capabilities'' {||} else let compl_batches = \<lambda>p t. map (de1 (os\<lparr>nfron := False\<rparr>) \<circ> fst) (filter (\<lambda>(d, t'). t' = t \<and> t \<in> set (filter (\<lambda>t. \<not> frontier_less_equal (front os p) t) (ocaps os p))) (input (os\<lparr>nfron := False\<rparr>) p)); ts = \<lambda>p. rmdups {} (map snd (filter (\<lambda>(d, t). t \<in> set (filter (\<lambda>t. \<not> frontier_less_equal (front os p) t) (ocaps os p))) (input (os\<lparr>nfron := False\<rparr>) p))); osa = os\<lparr>nfron := False, input := \<lambda>p. filter (\<lambda>(d, t). t \<notin> set (filter (\<lambda>t. \<not> frontier_less_equal (front os p) t) (ocaps os p))) (input (os\<lparr>nfron := False\<rparr>) p)\<rparr> in Let {|(concat (map (\<lambda>t. map (\<lambda>x. (x, Cap t 1)) (f (compl_batches 1 t))) (ts 1)), map (\<lambda>t. Cap t 1) (filter (\<lambda>t. \<not> frontier_less_equal (front os 1) t) (ocaps os 1)))|} ((|`|) (\<lambda>(outs, drops). trace (STR ''outs: '' + show_nat (length outs) + STR '' , drops: '' + show_nat (length drops)) (drop_caps (produces osa (map (\<lambda>(d, y). (en2 osa d, y)) outs)) drops))) else {||}))))))) op2'"
+    if "initia bt_state"
+      and "outpu bt_state 1 = (ab, bb) # xs"
+    for ab :: "'d1 + 'd2"
+      and bb :: 't
+      and xs :: "(('d1 + 'd2) \<times> 't) buf"
+    using that sorry
+  ultimately show ?thesis
+    apply -
+    unfolding R_def[symmetric]
+    subgoal premises prems2
+      apply (simp add: wsim_def dataflow_tree_to_operator_def batch_op_def batch_op_logic_def ooo_input_op_def notifier_op_def)
+      apply (intro allI conjI impI)
+      apply (elim step_builder_op_elim step_set_op_elim step_map_op_elim step_comp_op_elim step_dataflow_op_elim conjE ; 
+          clarsimp simp only: IO.simps ; hypsubst_thin ? ; clarsimp simp flip: cin.rep_eq split: option.splits sum.splits prod.splits if_splits ; hypsubst_thin?)
+      subgoal
+        using prems2(1) by assumption
+      subgoal
+        using prems2(2) by assumption
+      subgoal
+        using prems2(3) by assumption
+      subgoal
+        using prems2(4) by assumption
+      subgoal
+        using prems2(5) by assumption
+      subgoal
+        using prems2(6) by assumption
+      subgoal
+        using prems2(7) by assumption
+      subgoal
+        using prems2(8) by assumption
+      subgoal
+        using prems2(9) by assumption
+      subgoal
+        using prems2(10) by assumption
+      subgoal
+        using prems2(11) by assumption
+      done
+    done
+qed
+qed
 next
   case SIM2
   then show ?case sorry
