dataplane/Timely_Stream.thy
@@ -27,8 +27,27 @@ coinductive timely_productive where
 | "\<lbrakk>\<not> lfinite lxs; timely_productive lxs; ev_drops t 1 lxs \<rbrakk> \<Longrightarrow> timely_productive (LCons (Mint t) lxs)"
 | "\<lbrakk>\<not> lfinite lxs; timely_productive lxs \<rbrakk> \<Longrightarrow> timely_productive (LCons (Drop t) lxs)"
 
-
 definition "timely_input_stream lxs C =
  (timely_monotone lxs C \<and> (\<forall> t. ev_drops t (count C t) lxs) \<and> timely_productive lxs)"
+
+
+
+lemma
+  "Data t d \<in> lset lxs \<Longrightarrow> 
+   timely_input_stream lxs C \<Longrightarrow> 
+   lfinite (lfilter (case_event (\<lambda>t' d. t = t') (\<lambda>ta. False) (\<lambda>ta. False)) lxs)"
+  apply (induct lxs rule: lset_induct)
+  subgoal for lxs
+    unfolding timely_input_stream_def
+    apply (elim conjE)
+    apply (erule timely_productive.cases; simp; hypsubst_thin?)
+    subgoal for lxs'
+      apply (drule spec[of _ t])
+      apply (erule ev_drops.cases; simp; hypsubst_thin?)
+      subgoal
+        by (erule timely_monotone.cases; simp add: count_eq_zero_iff)
+      subgoal
+        apply (erule timely_monotone.cases; simp add: count_eq_zero_iff; hypsubst_thin?)
+        oops
 
 end
